src/simp/src/pureSimps.sig
@@ -1,0 +1,6 @@
+signature pureSimps = sig
+
+  val PURE_ss : simpLib.ssdata
+  val pure_ss : simpLib.simpset
+
+end
