src/bool/boolScript.sml
@@ -23,59 +23,59 @@ val _ = new_theory "bool";
 
 val EXISTS_DEF = define_exists();  (* Grandfather *)
 
-val T_DEF = 
+val T_DEF =
  new_definition
    ("T_DEF", Term `T = ((\x:bool. x) = \x:bool. x)`);
 
-val FORALL_DEF = 
- new_binder_definition 
+val FORALL_DEF =
+ new_binder_definition
    ("FORALL_DEF", Term `! = \P:'a->bool. P = \x. T`);
 
-val AND_DEF = 
+val AND_DEF =
  new_infix_definition
    ("AND_DEF",  Term `/\ = \t1. \t2. !t. (t1 ==> (t2 ==> t)) ==> t`, 400);
 
-val OR_DEF = 
+val OR_DEF =
  new_infix_definition
    ("OR_DEF", Term `\/ = \t1 t2. !t. (t1 ==> t) ==> ((t2 ==> t) ==> t)`, 300);
 
-val F_DEF = 
+val F_DEF =
  new_definition
    ("F_DEF", Term `F = !t. t`);
 
-val NOT_DEF = 
+val NOT_DEF =
  new_definition
    ("NOT_DEF", Term `~ = \t. t ==> F`);
 
-val EXISTS_UNIQUE_DEF = 
+val EXISTS_UNIQUE_DEF =
  new_binder_definition
    ("EXISTS_UNIQUE_DEF",
      Term `?! = \P:'a->bool. ($? P) /\ !x y. (P x /\ P y) ==> (x=y)`);
 
-val LET_DEF = 
+val LET_DEF =
  new_definition
    ("LET_DEF",  Term `LET = \(f:'a->'b) (x:'a). f x`);
 
-val COND_DEF = 
+val COND_DEF =
  new_definition
-   ("COND_DEF", Term `COND = \t t1 t2. @x:'a. ((t=T) ==> (x=t1)) /\ 
+   ("COND_DEF", Term `COND = \t t1 t2. @x:'a. ((t=T) ==> (x=t1)) /\
                                               ((t=F) ==> (x=t2))`);
 
-val ONE_ONE_DEF = 
+val ONE_ONE_DEF =
  new_definition
-   ("ONE_ONE_DEF", 
+   ("ONE_ONE_DEF",
       Term `ONE_ONE (f:'a->'b) = !x1 x2. (f x1 = f x2) ==> (x1 = x2)`);
 
-val ONTO_DEF = 
+val ONTO_DEF =
  new_definition
    ("ONTO_DEF", Term `ONTO (f:'a->'b) = !y.?x. y = f x`);
 
-val TYPE_DEFINITION = 
+val TYPE_DEFINITION =
  new_definition
    ("TYPE_DEFINITION",
-      Term `!P rep. TYPE_DEFINITION (P:'a->bool) (rep:'b->'a) 
+      Term `!P rep. TYPE_DEFINITION (P:'a->bool) (rep:'b->'a)
                     =
-                     (!x' x''. (rep x' = rep x'') ==> (x' = x'')) /\	
+                     (!x' x''. (rep x' = rep x'') ==> (x' = x'')) /\
                      (!x. P x = (?x'. x = rep x'))`);
 
 
@@ -83,23 +83,23 @@ val TYPE_DEFINITION =
  *                   AXIOMS                                                  *
  *---------------------------------------------------------------------------*)
 
-val BOOL_CASES_AX = 
+val BOOL_CASES_AX =
  new_axiom
    ("BOOL_CASES_AX", Term `!t:bool. (t=T) \/ (t=F)`);
 
-val IMP_ANTISYM_AX = 
+val IMP_ANTISYM_AX =
  new_axiom
    ("IMP_ANTISYM_AX", Term`!t1 t2. (t1 ==> t2) ==> (t2 ==> t1) ==> (t1 = t2)`);
 
-val ETA_AX = 
+val ETA_AX =
  new_axiom
    ("ETA_AX", Term `!t:'a->'b. (\x. t x) = t`);
 
-val SELECT_AX = 
+val SELECT_AX =
  new_axiom
    ("SELECT_AX", Term `!(P:'a->bool) x. P x ==> P ($@ P)`);
 
-val INFINITY_AX = 
+val INFINITY_AX =
  new_axiom
    ("INFINITY_AX",  Term `?f:ind->ind. ONE_ONE f /\ ~ONTO f`);
 
@@ -108,12 +108,12 @@ val INFINITY_AX =
 (*---------------------------------------------------------------------------*
  * Miscellaneous utility definitions, of use in some automated tools.        *
  *---------------------------------------------------------------------------*)
-val ARB_DEF = 
- new_definition 
+val ARB_DEF =
+ new_definition
    ("ARB_DEF",  Term `ARB = @x:'a. T`);
 
-val bool_case_DEF = 
- new_definition 
+val bool_case_DEF =
+ new_definition
    ("bool_case_DEF",  Term`bool_case (x:'a) y b = COND b x y`);
 
 
@@ -149,13 +149,13 @@ fun RAND_CONV conv tm =
    end;
 fun RATOR_CONV conv tm =
    let val {Rator,Rand} = dest_comb tm
-   in AP_THM (conv Rator) Rand 
+   in AP_THM (conv Rator) Rand
    end;
 fun RIGHT_BETA th = TRANS th (BETA_CONV(#rhs(dest_eq(concl th))));
 fun UNDISCH th = MP th (ASSUME(#ant(dest_imp(concl th))));
 fun CONJ_PAIR thm = (CONJUNCT1 thm, CONJUNCT2 thm);
 fun GENL varl thm = itlist GEN varl thm;
-fun SPECL tm_list th = rev_itlist SPEC tm_list th 
+fun SPECL tm_list th = rev_itlist SPEC tm_list th
 fun IMP_ANTISYM_RULE th1 th2 =
     let val {ant,conseq} = dest_imp(concl th1)
     in
@@ -163,60 +163,60 @@ fun IMP_ANTISYM_RULE th1 th2 =
     end
 
 (*---------------------------------------------------------------------------
- * |- !t. F ==> t  
+ * |- !t. F ==> t
  *---------------------------------------------------------------------------*)
 val FALSITY =
    let val t = --`t:bool`--
    in
-    GEN t (DISCH (--`F`--) 
+    GEN t (DISCH (--`F`--)
                  (SPEC t (EQ_MP F_DEF (ASSUME (--`F`--)))))
    end;
 
 val _ = save_thm("FALSITY", FALSITY);
 
-fun CONTR tm th = MP (SPEC tm FALSITY) th 
+fun CONTR tm th = MP (SPEC tm FALSITY) th
 
 fun DISJ_IMP dth =
    let val {disj1,disj2} = dest_disj (concl dth)
        val nota = mk_neg disj1
    in
      DISCH nota
-      (DISJ_CASES dth 
+      (DISJ_CASES dth
          (CONTR disj2 (MP (ASSUME nota) (ASSUME disj1)))
          (ASSUME disj2))
    end
 
-fun EQF_INTRO th = IMP_ANTISYM_RULE (NOT_ELIM th) 
+fun EQF_INTRO th = IMP_ANTISYM_RULE (NOT_ELIM th)
         (DISCH (Term`F`) (CONTR (dest_neg (concl th)) (ASSUME (Term`F`))));
 
 fun SELECT_EQ x =
  let val ty = type_of x
      val choose = mk_const{Name="@", Ty=(ty --> Type.bool) --> ty}
- in 
+ in
   fn th => AP_TERM choose (ABS x th)
  end
 
-fun GEN_ALL th = itlist GEN (set_diff (free_vars(concl th)) 
+fun GEN_ALL th = itlist GEN (set_diff (free_vars(concl th))
                                       (free_varsl (hyp th))) th;
 
 local fun f v (vs,l) = let val v' = variant vs v in (v'::vs, v'::l) end
 in
 fun SPEC_ALL th =
    let val (hvs,con) = (free_varsl ## I) (hyp th, concl th)
-       val fvs = free_vars con 
-       and vars = fst(strip_forall con) 
+       val fvs = free_vars con
+       and vars = fst(strip_forall con)
    in
      SPECL (snd(itlist f vars (hvs@fvs,[]))) th
    end
 end;
 
-fun CONJUNCTS th = 
+fun CONJUNCTS th =
   (CONJUNCTS (CONJUNCT1 th) @ CONJUNCTS (CONJUNCT2 th)) handle _ => [th];
 
-fun SUBST_CONV theta template tm = 
+fun SUBST_CONV theta template tm =
   let fun retheta {redex,residue} = (redex |-> genvar(type_of redex))
       val theta0 = map retheta theta
-      val theta1 = map2 (curry (op |->)) 
+      val theta1 = map2 (curry (op |->))
                         (map #residue theta0) (map #residue theta)
   in
    SUBST theta1 (mk_eq{lhs=tm,rhs=subst theta0 template}) (REFL tm)
@@ -239,9 +239,9 @@ fun SPEC_VAR th =
         val {lhs=a, rhs=b} = dest_eq (concl sth)
         val (abimp,baimp) = EQ_IMP_RULE sth
         fun HALF (p,q) pqimp =
-           let val xp = mk_exists{Bvar=x,Body=p} 
+           let val xp = mk_exists{Bvar=x,Body=p}
                and xq = mk_exists{Bvar=x,Body=q}
-           in DISCH xp 
+           in DISCH xp
                (CHOOSE (x, ASSUME xp) (EXISTS (xq,x) (MP pqimp (ASSUME p))))
            end
     in
@@ -256,7 +256,7 @@ fun SELECT_RULE th =
       val SELECT_AX' = INST_TYPE[alpha |-> type_of Bvar] SELECT_AX
       val th1 = SPEC v (SPEC P SELECT_AX')
       val {ant,conseq} = dest_imp(concl th1)
-      val th2 = BETA_CONV ant 
+      val th2 = BETA_CONV ant
       and th3 = BETA_CONV conseq
       val th4 = EQ_MP th3 (MP th1 (EQ_MP(SYM th2) (ASSUME (rhs(concl th2)))))
   in
@@ -285,7 +285,7 @@ fun EQT_INTRO th =
 
 
 (*---------------------------------------------------------------------------
- *  |- !t. t \/ ~t 
+ *  |- !t. t \/ ~t
  *---------------------------------------------------------------------------*)
 val EXCLUDED_MIDDLE =
    let val t = --`t:bool`--
@@ -313,7 +313,7 @@ fun IMP_ELIM th =
  *  |- !f y. (\x. f x) y = f y                                               *
  *---------------------------------------------------------------------------*)
 val BETA_THM =
-   GENL [Term`f:'a->'b`, Term `y:'a`] 
+   GENL [Term`f:'a->'b`, Term `y:'a`]
         (BETA_CONV (Term`(\x. (f:'a->'b) x) y`));
 
 val _ = save_thm("BETA_THM", BETA_THM);
@@ -322,13 +322,13 @@ val _ = save_thm("BETA_THM", BETA_THM);
  *  |- !t1:'a. !t2:'b. (\x. t1) t2 = t1                                      *
  *---------------------------------------------------------------------------*)
 val ABS_SIMP =
-   GENL [Term`t1:'a`, Term `t2:'b`] 
+   GENL [Term`t1:'a`, Term `t2:'b`]
         (BETA_CONV (Term`(\x:'b. t1:'a) t2`));
 
 val _ = save_thm("ABS_SIMP", ABS_SIMP);
 
 (*---------------------------------------------------------------------------
- *   |- !t. (!x.t)  =  t 
+ *   |- !t. (!x.t)  =  t
  *---------------------------------------------------------------------------*)
 val FORALL_SIMP =
  let val t = --`t:bool`--
@@ -342,14 +342,14 @@ val FORALL_SIMP =
 val _ = save_thm("FORALL_SIMP", FORALL_SIMP);
 
 (*---------------------------------------------------------------------------
- *   |- !t. (?x.t)  =  t  
+ *   |- !t. (?x.t)  =  t
  *---------------------------------------------------------------------------*)
 val EXISTS_SIMP =
    let val t = --`t:bool`--
        and x = --`x:'a`--
        val ext = --`?^x.^t`--
    in
-   GEN t (IMP_ANTISYM_RULE 
+   GEN t (IMP_ANTISYM_RULE
            (DISCH ext (CHOOSE((--`p:'a`--), ASSUME ext) (ASSUME t)))
            (DISCH t (EXISTS(ext, --`r:'a`--) (ASSUME t))))
    end;
@@ -393,7 +393,7 @@ val _ = save_thm("AND1_THM", AND1_THM);
 
 
 (*---------------------------------------------------------------------------
- *    |- !t1 t2. t1 /\ t2 ==> t2 
+ *    |- !t1 t2. t1 /\ t2 ==> t2
  *---------------------------------------------------------------------------*)
 val AND2_THM =
   let val t1 = --`t1:bool`--
@@ -409,7 +409,7 @@ val AND2_THM =
 val _ = save_thm("AND2_THM", AND2_THM);
 
 (*---------------------------------------------------------------------------
- *   |- !t1 t2. (t1 /\ t2) = (t2 /\ t1)  
+ *   |- !t1 t2. (t1 /\ t2) = (t2 /\ t1)
  *---------------------------------------------------------------------------*)
 val CONJ_SYM =
   let val t1 = --`t1:bool`--
@@ -427,7 +427,7 @@ val CONJ_SYM =
 val _ = save_thm("CONJ_SYM", CONJ_SYM);
 
 (*---------------------------------------------------------------------------
- * |- !t1 t2 t3. t1 /\ (t2 /\ t3) = (t1 /\ t2) /\ t3 
+ * |- !t1 t2 t3. t1 /\ (t2 /\ t3) = (t1 /\ t2) /\ t3
  *---------------------------------------------------------------------------*)
 val CONJ_ASSOC =
   let val t1 = --`t1:bool`--
@@ -451,7 +451,7 @@ val _ = save_thm("CONJ_ASSOC", CONJ_ASSOC);
 
 
 (*---------------------------------------------------------------------------
- *  |- !t1 t2. t1 ==> t1 \/ t2 
+ *  |- !t1 t2. t1 ==> t1 \/ t2
  *---------------------------------------------------------------------------*)
 val OR_INTRO_THM1 =
   let val t = --`t:bool`--
@@ -468,13 +468,13 @@ val OR_INTRO_THM1 =
 val _ = save_thm("OR_INTRO_THM1", OR_INTRO_THM1);
 
 (*---------------------------------------------------------------------------
- * |- !t1 t2. t2 ==> t1 \/ t2 
+ * |- !t1 t2. t2 ==> t1 \/ t2
  *---------------------------------------------------------------------------*)
 val OR_INTRO_THM2 =
   let val t  = --`t:bool`--
       and t1 = --`t1:bool`--
       and t2 = --`t2:bool`--
-      val th1 = ADD_ASSUM (--`^t1 ==> ^t`--) 
+      val th1 = ADD_ASSUM (--`^t1 ==> ^t`--)
                      (MP (ASSUME (--`^t2 ==> ^t`--)) (ASSUME t2))
       val th2 = GEN t (DISCH (--`^t1 ==> ^t`--) (DISCH (--`^t2 ==> ^t`--) th1))
       val th3 = RIGHT_BETA(AP_THM (RIGHT_BETA(AP_THM OR_DEF t1)) t2)
@@ -505,13 +505,13 @@ val _ = save_thm("OR_ELIM_THM", OR_ELIM_THM);
 
 
 (*---------------------------------------------------------------------------
- * |- !t. (t ==> F) ==> ~t 
+ * |- !t. (t ==> F) ==> ~t
  *---------------------------------------------------------------------------*)
 val IMP_F =
    let val t = --`t:bool`--
        val th1 = RIGHT_BETA (AP_THM NOT_DEF t)
    in
-     GEN t (DISCH (--`^t ==> F`--) 
+     GEN t (DISCH (--`^t ==> F`--)
                  (EQ_MP (SYM th1) (ASSUME (--`^t ==> F`--))))
    end;
 
@@ -519,13 +519,13 @@ val _ = save_thm("IMP_F", IMP_F);
 
 
 (*---------------------------------------------------------------------------
- * |- !t. ~t ==> (t ==> F)  
+ * |- !t. ~t ==> (t ==> F)
  *---------------------------------------------------------------------------*)
 val F_IMP =
    let val t = --`t:bool`--
        val th1 = RIGHT_BETA(AP_THM NOT_DEF t)
    in
-   GEN t (DISCH (--`~^t`--) 
+   GEN t (DISCH (--`~^t`--)
                 (EQ_MP th1 (ASSUME (--`~^t`--))))
    end;
 
@@ -533,7 +533,7 @@ val _ = save_thm("F_IMP", F_IMP);
 
 
 (*---------------------------------------------------------------------------
- * |- !t. ~t ==> (t=F) 
+ * |- !t. ~t ==> (t=F)
  *---------------------------------------------------------------------------*)
 val NOT_F =
    let val t = --`t:bool`--
@@ -547,7 +547,7 @@ val NOT_F =
 val _ = save_thm("NOT_F", NOT_F);
 
 (*---------------------------------------------------------------------------
- *  |- !t. ~(t /\ ~t)  
+ *  |- !t. ~(t /\ ~t)
  *---------------------------------------------------------------------------*)
 
 val NOT_AND =
@@ -559,7 +559,7 @@ val _ = save_thm("NOT_AND", NOT_AND);
 
 
 (*---------------------------------------------------------------------------
- * |- !t. (T /\ t) = t 
+ * |- !t. (T /\ t) = t
  *---------------------------------------------------------------------------*)
 val AND_CLAUSE1 =
    let val t = --`t:bool`--
@@ -571,7 +571,7 @@ val AND_CLAUSE1 =
 
 
 (*---------------------------------------------------------------------------
- *  |- !t. (t /\ T) = t 
+ *  |- !t. (t /\ T) = t
  *---------------------------------------------------------------------------*)
 val AND_CLAUSE2 =
    let val t = --`t:bool`--
@@ -583,11 +583,11 @@ val AND_CLAUSE2 =
 
 
 (*---------------------------------------------------------------------------
- *   |- !t. (F /\ t) = F 
+ *   |- !t. (F /\ t) = F
  *---------------------------------------------------------------------------*)
 val AND_CLAUSE3 =
    let val t = --`t:bool`--
-       val th1 = IMP_TRANS (SPEC t (SPEC (--`F`--) AND1_THM)) 
+       val th1 = IMP_TRANS (SPEC t (SPEC (--`F`--) AND1_THM))
                            (SPEC (--`F`--) FALSITY)
        and th2 = SPEC (--`F /\ ^t`--) FALSITY
    in
@@ -595,11 +595,11 @@ val AND_CLAUSE3 =
    end;
 
 (*---------------------------------------------------------------------------
- *   |- !t. (t /\ F) = F 
+ *   |- !t. (t /\ F) = F
  *---------------------------------------------------------------------------*)
 val AND_CLAUSE4 =
    let val t = --`t:bool`--
-       val th1 = IMP_TRANS (SPEC (--`F`--) (SPEC t AND2_THM)) 
+       val th1 = IMP_TRANS (SPEC (--`F`--) (SPEC t AND2_THM))
                            (SPEC (--`F`--) FALSITY)
        and th2 = SPEC (--`^t /\ F`--) FALSITY
    in
@@ -608,7 +608,7 @@ val AND_CLAUSE4 =
 
 
 (*---------------------------------------------------------------------------
- *    |- !t. (t /\ t) = t 
+ *    |- !t. (t /\ t) = t
  *---------------------------------------------------------------------------*)
 val AND_CLAUSE5 =
    let val t = --`t:bool`--
@@ -628,20 +628,20 @@ val AND_CLAUSE5 =
 val AND_CLAUSES =
    let val t = --`t:bool`--
    in
-   GEN t (CONJ 
+   GEN t (CONJ
            (SPEC t AND_CLAUSE1)
             (CONJ
              (SPEC t AND_CLAUSE2)
               (CONJ
                (SPEC t AND_CLAUSE3)
-                 (CONJ (SPEC t AND_CLAUSE4) 
+                 (CONJ (SPEC t AND_CLAUSE4)
                        (SPEC t AND_CLAUSE5)))))
    end;
 
 val _ = save_thm("AND_CLAUSES", AND_CLAUSES);
 
 (*---------------------------------------------------------------------------
- *   |- !t. (T \/ t) = T 
+ *   |- !t. (T \/ t) = T
  *---------------------------------------------------------------------------*)
 val OR_CLAUSE1 =
    let val t = --`t:bool`--
@@ -652,7 +652,7 @@ val OR_CLAUSE1 =
    end;
 
 (*---------------------------------------------------------------------------
- *  |- !t. (t \/ T) = T 
+ *  |- !t. (t \/ T) = T
  *---------------------------------------------------------------------------*)
 val OR_CLAUSE2 =
    let val t = --`t:bool`--
@@ -663,7 +663,7 @@ val OR_CLAUSE2 =
    end;
 
 (*---------------------------------------------------------------------------
- *    |- (F \/ t) = t 
+ *    |- (F \/ t) = t
  *---------------------------------------------------------------------------*)
 val OR_CLAUSE3 =
    let val t = --`t:bool`--
@@ -689,11 +689,11 @@ val OR_CLAUSE4 =
    end;
 
 (*---------------------------------------------------------------------------
- *   |- !t. (t \/ t) = t 
+ *   |- !t. (t \/ t) = t
  *---------------------------------------------------------------------------*)
 val OR_CLAUSE5 =
    let val t = --`t:bool`--
-       val th1 = DISCH (--`^t \/ ^t`--) 
+       val th1 = DISCH (--`^t \/ ^t`--)
                   (DISJ_CASES(ASSUME (--`^t \/ ^t`--)) (ASSUME t) (ASSUME t))
        and th2 = DISCH t (DISJ1(ASSUME t)t)
    in
@@ -710,13 +710,13 @@ val OR_CLAUSE5 =
 val OR_CLAUSES =
    let val t = --`t:bool`--
    in
-   GEN t (CONJ 
+   GEN t (CONJ
           (SPEC t OR_CLAUSE1)
           (CONJ
            (SPEC t OR_CLAUSE2)
-           (CONJ 
+           (CONJ
             (SPEC t OR_CLAUSE3)
-            (CONJ (SPEC t OR_CLAUSE4) 
+            (CONJ (SPEC t OR_CLAUSE4)
                   (SPEC t OR_CLAUSE5)))))
    end;
 
@@ -724,7 +724,7 @@ val _ = save_thm("OR_CLAUSES", OR_CLAUSES);
 
 
 (*---------------------------------------------------------------------------
- *  |- !t. (T ==> t) = t  
+ *  |- !t. (T ==> t) = t
  *---------------------------------------------------------------------------*)
 val IMP_CLAUSE1 =
    let val t = --`t:bool`--
@@ -736,7 +736,7 @@ val IMP_CLAUSE1 =
    end;
 
 (*---------------------------------------------------------------------------
- *  |- !t. (F ==> t) = T 
+ *  |- !t. (F ==> t) = T
  *---------------------------------------------------------------------------*)
 val IMP_CLAUSE2 =
    let val t = --`t:bool`--
@@ -745,7 +745,7 @@ val IMP_CLAUSE2 =
    end;
 
 (*---------------------------------------------------------------------------
- *  |- !t. (t ==> T) = T 
+ *  |- !t. (t ==> T) = T
  *---------------------------------------------------------------------------*)
 val IMP_CLAUSE3 =
    let val t = --`t:bool`--
@@ -754,7 +754,7 @@ val IMP_CLAUSE3 =
    end;
 
 (*---------------------------------------------------------------------------
- *  |- ((T ==> F) = F) /\ ((F ==> F) = T) 
+ *  |- ((T ==> F) = F) /\ ((F ==> F) = T)
  *---------------------------------------------------------------------------*)
 val IMP_CLAUSE4 =
    let val th1 = DISCH (--`T ==> F`--) (MP (ASSUME (--`T ==> F`--)) TRUTH)
@@ -766,7 +766,7 @@ val IMP_CLAUSE4 =
    end;
 
 (*---------------------------------------------------------------------------
- *  |- !t. (t ==> F) = ~t 
+ *  |- !t. (t ==> F) = ~t
  *---------------------------------------------------------------------------*)
 val IMP_CLAUSE5 =
     let val t = --`t:bool`--
@@ -797,7 +797,7 @@ val _ = save_thm("IMP_CLAUSES", IMP_CLAUSES);
 
 
 (*----------------------------------------------------------------------------
- *    |- (~~t = t) /\ (~T = F) /\ (~F = T) 
+ *    |- (~~t = t) /\ (~T = F) /\ (~F = T)
  *---------------------------------------------------------------------------*)
 val NOT_CLAUSES =
  CONJ
@@ -807,7 +807,7 @@ val NOT_CLAUSES =
       (DISCH (--`t:bool`--)
        (NOT_INTRO(DISCH (--`~t`--) (UNDISCH (NOT_ELIM(ASSUME (--`~t`--)))))))))
   (CONJ (IMP_ANTISYM_RULE
-          (DISCH (--`~T`--) 
+          (DISCH (--`~T`--)
                  (MP (MP (SPEC (--`T`--) F_IMP) (ASSUME (--`~T`--))) TRUTH))
           (SPEC (--`~T`--) FALSITY))
         (IMP_ANTISYM_RULE (DISCH (--`~F`--) TRUTH)
@@ -817,21 +817,21 @@ val NOT_CLAUSES =
 val _ = save_thm("NOT_CLAUSES", NOT_CLAUSES);
 
 (*---------------------------------------------------------------------------
- *   |- !x. x=x 
+ *   |- !x. x=x
  *---------------------------------------------------------------------------*)
 val EQ_REFL = GEN (--`x : 'a`--) (REFL (--`x : 'a`--));
 
 val _ = save_thm("EQ_REFL", EQ_REFL);
 
 (*---------------------------------------------------------------------------
- *   |- !x. (x=x) = T 
+ *   |- !x. (x=x) = T
  *---------------------------------------------------------------------------*)
 val REFL_CLAUSE = GEN (--`x: 'a`--) (EQT_INTRO(SPEC (--`x:'a`--) EQ_REFL));
 
 val _ = save_thm("REFL_CLAUSE", REFL_CLAUSE );
 
 (*---------------------------------------------------------------------------
- *   |- !x y. x=y  ==>  y=x  
+ *   |- !x y. x=y  ==>  y=x
  *---------------------------------------------------------------------------*)
 val EQ_SYM =
  let val x = --`x:'a`--
@@ -847,14 +847,14 @@ val _ = save_thm("EQ_SYM",EQ_SYM);
  *---------------------------------------------------------------------------*)
 val EQ_SYM_EQ =
    GEN (--`x:'a`--)
-    (GEN (--`y:'a`--) 
+    (GEN (--`y:'a`--)
       (IMP_ANTISYM_RULE (SPEC (--`y:'a`--) (SPEC (--`x:'a`--) EQ_SYM))
                         (SPEC (--`x:'a`--) (SPEC (--`y:'a`--) EQ_SYM))));
 
 val _ = save_thm("EQ_SYM_EQ",EQ_SYM_EQ);
 
 (*---------------------------------------------------------------------------
- *    |- !f g. (!x. f x = g x)  ==>  f=g 
+ *    |- !f g. (!x. f x = g x)  ==>  f=g
  *---------------------------------------------------------------------------*)
 val EQ_EXT =
    let val f = (--`f:'a->'b`--)
@@ -867,7 +867,7 @@ val EQ_EXT =
 val _ = save_thm("EQ_EXT",EQ_EXT);
 
 (*---------------------------------------------------------------------------
- *    |- !x y z. x=y  /\  y=z  ==>  x=z 
+ *    |- !x y z. x=y  /\  y=z  ==>  x=z
  *---------------------------------------------------------------------------*)
 val EQ_TRANS =
    let val x = --`x:'a`--
@@ -879,14 +879,14 @@ val EQ_TRANS =
     (GEN y
      (GEN z
       (DISCH xyyz
-       (TRANS (CONJUNCT1(ASSUME xyyz)) 
+       (TRANS (CONJUNCT1(ASSUME xyyz))
               (CONJUNCT2(ASSUME xyyz))))))
    end;
 
 val _ = save_thm("EQ_TRANS",EQ_TRANS);
 
 (*---------------------------------------------------------------------------
- *     |- ~(T=F) /\ ~(F=T) 
+ *     |- ~(T=F) /\ ~(F=T)
  *---------------------------------------------------------------------------*)
 val BOOL_EQ_DISTINCT =
    let val TF = --`T = F`--
@@ -914,7 +914,7 @@ val EQ_CLAUSE1 =
 
 
 (*---------------------------------------------------------------------------
- *  |- !t. (t = T) = t 
+ *  |- !t. (t = T) = t
  *---------------------------------------------------------------------------*)
 val EQ_CLAUSE2 =
    let val t = --`t:bool`--
@@ -925,9 +925,9 @@ val EQ_CLAUSE2 =
    GEN t (IMP_ANTISYM_RULE th1 th2)
    end;
 
- 
+
 (*---------------------------------------------------------------------------
- *    |- !t. (F = t) = ~t 
+ *    |- !t. (F = t) = ~t
  *---------------------------------------------------------------------------*)
 val EQ_CLAUSE3 =
    let val t = --`t:bool`--
@@ -944,7 +944,7 @@ val EQ_CLAUSE3 =
 
 
 (*---------------------------------------------------------------------------
- *  |- !t. (t = F) = ~t 
+ *  |- !t. (t = F) = ~t
  *---------------------------------------------------------------------------*)
 val EQ_CLAUSE4 =
    let val t = --`t:bool`--
@@ -956,7 +956,7 @@ val EQ_CLAUSE4 =
    in
    GEN t (IMP_ANTISYM_RULE th1 th2)
    end;
- 
+
 
 (*---------------------------------------------------------------------------
  *  |- !t.  (T = t)  =  t  /\
@@ -979,21 +979,21 @@ val _ = save_thm("EQ_CLAUSES", EQ_CLAUSES);
 
 
 (*---------------------------------------------------------------------------
- *    |- !t1 t2 :'a. COND T t1 t2 = t1 
+ *    |- !t1 t2 :'a. COND T t1 t2 = t1
  *---------------------------------------------------------------------------*)
 val COND_CLAUSE1 =
- let val (x,t1,t2,v) = (Term`x:'a`, Term`t1:'a`, 
+ let val (x,t1,t2,v) = (Term`x:'a`, Term`t1:'a`,
                         Term`t2:'a`, genvar Type.bool)
      val th1 = RIGHT_BETA(AP_THM
                  (RIGHT_BETA(AP_THM
                     (RIGHT_BETA(AP_THM COND_DEF (--`T`--))) t1))t2)
      val TT = EQT_INTRO(REFL (--`T`--))
-     val th2 = SUBST [v |-> SYM TT] 
-                     (--`(^v ==> (^x=^t1)) = (^x=^t1)`--) 
+     val th2 = SUBST [v |-> SYM TT]
+                     (--`(^v ==> (^x=^t1)) = (^x=^t1)`--)
                      (CONJUNCT1 (SPEC (--`^x=^t1`--) IMP_CLAUSES))
      and th3 = DISCH (--`T=F`--)
                      (MP (SPEC (--`^x=^t2`--) FALSITY)
-                         (UNDISCH(MP (SPEC (--`T=F`--) F_IMP) 
+                         (UNDISCH(MP (SPEC (--`T=F`--) F_IMP)
                                      (CONJUNCT1 BOOL_EQ_DISTINCT))))
      val th4 = DISCH (--`^x=^t1`--)
                      (CONJ(EQ_MP(SYM th2)(ASSUME (--`^x=^t1`--)))th3)
@@ -1001,7 +1001,7 @@ val COND_CLAUSE1 =
                      (MP (CONJUNCT1(ASSUME (--`((T=T) ==> (^x=^t1))/\
                                                ((T=F) ==> (^x=^t2))`--)))
                          (REFL (--`T`--)))
-     val th6 = MP (MP (SPEC (--`((T=T) ==> (^x=^t1))/\((T=F) ==> (^x=^t2))`--) 
+     val th6 = MP (MP (SPEC (--`((T=T) ==> (^x=^t1))/\((T=F) ==> (^x=^t2))`--)
                             (SPEC (--`^x=^t1`--) IMP_ANTISYM_AX))
                       th4)
                   th5
@@ -1014,14 +1014,14 @@ val COND_CLAUSE1 =
 
 
 (*---------------------------------------------------------------------------
- *    |- !tm1 tm2:'a. COND F tm1 tm2 = tm2 
+ *    |- !tm1 tm2:'a. COND F tm1 tm2 = tm2
  *
  *   Note that there is a bound variable conflict if we use use t1
- *   and t2 as the variable names. That would be a good test of the 
+ *   and t2 as the variable names. That would be a good test of the
  *   substitution algorithm.
  *---------------------------------------------------------------------------*)
 val COND_CLAUSE2 =
-   let val (x,t1,t2,v) = (--`x:'a`--,  --`tm1:'a`--, --`tm2:'a`--, 
+   let val (x,t1,t2,v) = (--`x:'a`--,  --`tm1:'a`--, --`tm2:'a`--,
                           genvar (==`:bool`==))
        val th1 = RIGHT_BETA(AP_THM
                    (RIGHT_BETA(AP_THM
@@ -1031,7 +1031,7 @@ val COND_CLAUSE2 =
                        (--`(^v ==> (^x=^t2))=(^x=^t2)`--)
                        (CONJUNCT1(SPEC (--`^x=^t2`--) IMP_CLAUSES))
        and th3 = DISCH (--`F=T`--) (MP (SPEC (--`^x=^t1`--) FALSITY)
-                                 (UNDISCH (MP (SPEC (--`F=T`--) F_IMP) 
+                                 (UNDISCH (MP (SPEC (--`F=T`--) F_IMP)
                                               (CONJUNCT2 BOOL_EQ_DISTINCT))))
        val th4 = DISCH (--`^x=^t2`--)
                        (CONJ th3 (EQ_MP(SYM th2)(ASSUME (--`^x=^t2`--))))
@@ -1054,7 +1054,7 @@ val COND_CLAUSE2 =
 
 
 (*---------------------------------------------------------------------------
- *    |- !t1:'a.!t2:'a. ((T => t1 | t2) = t1) /\ ((F => t1 | t2) = t2) 
+ *    |- !t1:'a.!t2:'a. ((T => t1 | t2) = t1) /\ ((F => t1 | t2) = t2)
  *---------------------------------------------------------------------------*)
 val COND_CLAUSES =
    let val (t1,t2) = (--`t1:'a`--, --`t2:'a`--)
@@ -1075,14 +1075,14 @@ val COND_ID =
    let val b = --`b:bool`--
        and t = --`t:'a`--
        val def = INST_TYPE [==`:'b`==  |->  ==`:'a`==] COND_DEF
-       val th1 = itlist (fn x => RIGHT_BETA o (C AP_THM x)) 
+       val th1 = itlist (fn x => RIGHT_BETA o (C AP_THM x))
                         [t,t,b] def
        val p = genvar (==`:bool`==)
        val asm1 = ASSUME (--`((^b=T)==>^p) /\ ((^b=F)==>^p)`--)
        val th2 = DISJ_CASES (SPEC b BOOL_CASES_AX)
                             (UNDISCH (CONJUNCT1 asm1))
                             (UNDISCH (CONJUNCT2 asm1))
-       val imp1 = DISCH (concl asm1) th2 
+       val imp1 = DISCH (concl asm1) th2
        val asm2 = ASSUME p
        val imp2 = DISCH p (CONJ (DISCH (--`^b=T`--)
                                        (ADD_ASSUM (--`^b=T`--) asm2))
@@ -1094,7 +1094,7 @@ val COND_ID =
        val th4 = EQ_MP (SYM(BETA_CONV (--`(\x.x = ^t) ^t`--)))
                        (REFL t)
        val th5 = MP (SPEC t (SPEC (--`\x.x = ^t` --) SELECT_AX)) th4
-       val lemma2 = EQ_MP (BETA_CONV(concl th5)) th5 
+       val lemma2 = EQ_MP (BETA_CONV(concl th5)) th5
    in
      GEN b (GEN t (TRANS th3 lemma2))
    end;
@@ -1106,12 +1106,12 @@ val _ = save_thm("COND_ID", COND_ID);
 (* ---------------------------------------------------------------------*)
 
 val SELECT_REFL =
-  let val th1 = SPEC (--`x:'a`--) 
+  let val th1 = SPEC (--`x:'a`--)
                       (SPEC (--`\y:'a. y = x`--) SELECT_AX)
-      val ths = map BETA_CONV [--`(\y:'a. y = x) x`--, 
+      val ths = map BETA_CONV [--`(\y:'a. y = x) x`--,
                                --`(\y:'a. y = x)(@y. y = x)`--]
       val th2 = SUBST[Term`u:bool` |-> el 1 ths, Term`v:bool` |-> el 2 ths]
-                     (Term`u ==> v`) th1 
+                     (Term`u ==> v`) th1
   in
   GEN (--`x:'a`--) (MP th2 (REFL (--`x:'a`--)))
   end;
@@ -1131,9 +1131,9 @@ val SELECT_UNIQUE =
       val th3 = AP_TERM (--`$@ :('a->bool)->'a`--) th2
       val th4 = TRANS (BETA_CONV (--`(\y:'a. y = x) y`--)) th0
       val th5 = AP_TERM (--`$@ :('a->bool)->'a`--) (EXT(GEN (--`y:'a`--) th4))
-      val th6 = TRANS (TRANS th3 (SYM th5)) (SPEC (--`x:'a`--) SELECT_REFL) 
+      val th6 = TRANS (TRANS th3 (SYM th5)) (SPEC (--`x:'a`--) SELECT_REFL)
   in
-  GENL [(--`P:'a->bool`--), (--`x:'a`--)] 
+  GENL [(--`P:'a->bool`--), (--`x:'a`--)]
        (DISCH (--`!y:'a. P y = (y = x)`--) th6)
   end;
 
@@ -1146,45 +1146,45 @@ val _ = save_thm("SELECT_UNIQUE", SELECT_UNIQUE);
 val NOT_FORALL_THM =
     let val f = (--`P:'a->bool`--)
 	val x = (--`x:'a`--)
-	val t = mk_comb{Rator=f,Rand=x} 
+	val t = mk_comb{Rator=f,Rand=x}
 	val all = mk_forall{Bvar=x,Body=t}
 	and exists = mk_exists{Bvar=x,Body=mk_neg t}
-	val nott = ASSUME (mk_neg t) 
-	val th1 = DISCH all (MP nott (SPEC x (ASSUME all))) 
-	val imp1 = DISCH exists (CHOOSE (x, ASSUME exists) (NOT_INTRO th1)) 
+	val nott = ASSUME (mk_neg t)
+	val th1 = DISCH all (MP nott (SPEC x (ASSUME all)))
+	val imp1 = DISCH exists (CHOOSE (x, ASSUME exists) (NOT_INTRO th1))
 	val th2 =
-	    CCONTR t (MP (ASSUME(mk_neg exists)) (EXISTS(exists,x)nott)) 
-	val th3 = CCONTR exists (MP (ASSUME (mk_neg all)) (GEN x th2)) 
-	val imp2 = DISCH (mk_neg all) th3 
+	    CCONTR t (MP (ASSUME(mk_neg exists)) (EXISTS(exists,x)nott))
+	val th3 = CCONTR exists (MP (ASSUME (mk_neg all)) (GEN x th2))
+	val imp2 = DISCH (mk_neg all) th3
     in
 	GEN f (IMP_ANTISYM_RULE imp2 imp1)
     end;
 
 val _ = save_thm("NOT_FORALL_THM",NOT_FORALL_THM);
-    
+
 
 (* ------------------------------------------------------------------------- *)
 (* NOT_EXISTS_THM = |- !P. ~(?x. P x) = (!x. ~P x)                   	    *)
 (* ------------------------------------------------------------------------- *)
 
 val NOT_EXISTS_THM =
-    let val f = (--`P:'a->bool`--) 
-	val x = (--`x:'a`--) 
-	val t = mk_comb{Rator=f,Rand=x} 
-	val tm = mk_neg(mk_exists{Bvar=x,Body=t}) 
-	val all = mk_forall{Bvar=x,Body=mk_neg t} 
-	val asm1 = ASSUME t 
-	val thm1 = MP (ASSUME tm) (EXISTS (rand tm, x) asm1) 
-	val imp1 = DISCH tm (GEN x (NOT_INTRO (DISCH t thm1))) 
-	val asm2 = ASSUME  all and asm3 = ASSUME (rand tm) 
-	val thm2 = DISCH (rand tm) (CHOOSE (x,asm3) (MP (SPEC x asm2) asm1)) 
-	val imp2 = DISCH all (NOT_INTRO thm2) 
+    let val f = (--`P:'a->bool`--)
+	val x = (--`x:'a`--)
+	val t = mk_comb{Rator=f,Rand=x}
+	val tm = mk_neg(mk_exists{Bvar=x,Body=t})
+	val all = mk_forall{Bvar=x,Body=mk_neg t}
+	val asm1 = ASSUME t
+	val thm1 = MP (ASSUME tm) (EXISTS (rand tm, x) asm1)
+	val imp1 = DISCH tm (GEN x (NOT_INTRO (DISCH t thm1)))
+	val asm2 = ASSUME  all and asm3 = ASSUME (rand tm)
+	val thm2 = DISCH (rand tm) (CHOOSE (x,asm3) (MP (SPEC x asm2) asm1))
+	val imp2 = DISCH all (NOT_INTRO thm2)
     in
 	GEN f (IMP_ANTISYM_RULE imp1 imp2)
     end;
 
 val _ = save_thm("NOT_EXISTS_THM",NOT_EXISTS_THM);
-    
+
 
 (* ------------------------------------------------------------------------- *)
 (* FORALL_AND_THM |- !P Q. (!x. P x /\ Q x) = ((!x. P x) /\ (!x. Q x))       *)
@@ -1196,16 +1196,16 @@ val FORALL_AND_THM =
 	val x = (--`x:'a`--)
 	val th1 = ASSUME (--`!x:'a. (P x) /\ (Q x)`--)
 	val imp1 =
-	    (uncurry CONJ) ((GEN x ## GEN x) (CONJ_PAIR (SPEC x th1))) 
+	    (uncurry CONJ) ((GEN x ## GEN x) (CONJ_PAIR (SPEC x th1)))
 	val th2 = ASSUME (--`(!x:'a. P x) /\ (!x:'a. Q x)`--)
 	val imp2 =
 	    GEN x (uncurry CONJ ((SPEC x ## SPEC x) (CONJ_PAIR th2)))
     in
 	    GENL [f,g] (IMP_ANTISYM_RULE (DISCH_ALL imp1) (DISCH_ALL imp2))
     end;
-    
+
 val _ = save_thm("FORALL_AND_THM",FORALL_AND_THM);
-    
+
 
 
 (* ------------------------------------------------------------------------- *)
@@ -1213,38 +1213,38 @@ val _ = save_thm("FORALL_AND_THM",FORALL_AND_THM);
 (* ------------------------------------------------------------------------- *)
 
 val LEFT_AND_FORALL_THM =
-    let val x = (--`x:'a`--) 
-	val f = (--`P:'a->bool`--) 
-	val Q = (--`Q:bool`--) 
-	val th1 = ASSUME (--`(!x:'a. P x) /\ Q`--) 
-	val imp1 = GEN x ((uncurry CONJ) ((SPEC x ## I) (CONJ_PAIR th1))) 
-	val th2 = ASSUME (--`!x:'a. P x /\ Q`--) 
+    let val x = (--`x:'a`--)
+	val f = (--`P:'a->bool`--)
+	val Q = (--`Q:bool`--)
+	val th1 = ASSUME (--`(!x:'a. P x) /\ Q`--)
+	val imp1 = GEN x ((uncurry CONJ) ((SPEC x ## I) (CONJ_PAIR th1)))
+	val th2 = ASSUME (--`!x:'a. P x /\ Q`--)
 	val imp2 = (uncurry CONJ) ((GEN x ## I) (CONJ_PAIR (SPEC x th2)))
     in
 	GENL [f,Q] (IMP_ANTISYM_RULE (DISCH_ALL imp1) (DISCH_ALL imp2))
     end;
 
 val _ = save_thm("LEFT_AND_FORALL_THM",LEFT_AND_FORALL_THM);
-    
+
 
 (* ------------------------------------------------------------------------- *)
 (* RIGHT_AND_FORALL_THM = |- !P Q. P /\ (!x. Q x) = (!x. P /\ Q x)           *)
 (* ------------------------------------------------------------------------- *)
 
 val RIGHT_AND_FORALL_THM =
-    let	val x = (--`x:'a`--) 
-	val P = (--`P:bool`--) 
-	val g = (--`Q:'a->bool`--) 
-	val th1 = ASSUME (--`P /\ (!x:'a. Q x)`--) 
-	val imp1 = GEN x ((uncurry CONJ) ((I ## SPEC x) (CONJ_PAIR th1))) 
-	val th2 = ASSUME (--`!x:'a. P /\ Q x`--) 
-	val imp2 = (uncurry CONJ) ((I ## GEN x) (CONJ_PAIR (SPEC x th2))) 
+    let	val x = (--`x:'a`--)
+	val P = (--`P:bool`--)
+	val g = (--`Q:'a->bool`--)
+	val th1 = ASSUME (--`P /\ (!x:'a. Q x)`--)
+	val imp1 = GEN x ((uncurry CONJ) ((I ## SPEC x) (CONJ_PAIR th1)))
+	val th2 = ASSUME (--`!x:'a. P /\ Q x`--)
+	val imp2 = (uncurry CONJ) ((I ## GEN x) (CONJ_PAIR (SPEC x th2)))
     in
 	GENL [P,g] (IMP_ANTISYM_RULE (DISCH_ALL imp1) (DISCH_ALL imp2))
     end;
 
 val _ = save_thm("RIGHT_AND_FORALL_THM",RIGHT_AND_FORALL_THM);
-    
+
 
 (* ------------------------------------------------------------------------- *)
 (* EXISTS_OR_THM |- !P Q. (?x. P x \/ Q x) = ((?x. P x) \/ (?x. Q x))        *)
@@ -1267,13 +1267,13 @@ val EXISTS_OR_THM =
 	val th1 = EXISTS(tm,x) t1 and th2 = EXISTS(tm,x) t2
 	val e1 = CHOOSE (x,ASSUME ep) th1 and e2 = CHOOSE (x,ASSUME eq) th2
 	val thm2 = DISJ_CASES (ASSUME(mk_disj{disj1=ep,disj2=eq})) e1 e2
-	val imp2 = DISCH (mk_disj{disj1=ep,disj2=eq}) thm2 
+	val imp2 = DISCH (mk_disj{disj1=ep,disj2=eq}) thm2
     in
 	GENL [f,g] (IMP_ANTISYM_RULE imp1 imp2)
     end;
 
 val _ = save_thm("EXISTS_OR_THM",EXISTS_OR_THM);
-    
+
 
 (* ------------------------------------------------------------------------- *)
 (* LEFT_OR_EXISTS_THM = |- (?x. P x) \/ Q = (?x. P x \/ Q)                   *)
@@ -1288,18 +1288,18 @@ val LEFT_OR_EXISTS_THM =
 	val tm = mk_disj{disj1=ep,disj2=Q}
 	val otm = mk_exists{Bvar=x,Body=mk_disj{disj1=P,disj2=Q}}
 	val t1 = DISJ1 (ASSUME P) Q and t2 = DISJ2 P (ASSUME Q)
-	val th1 = EXISTS(otm,x) t1 and th2 = EXISTS(otm,x) t2 
+	val th1 = EXISTS(otm,x) t1 and th2 = EXISTS(otm,x) t2
 	val thm1 = DISJ_CASES (ASSUME tm) (CHOOSE(x,ASSUME ep)th1) th2
 	val imp1 = DISCH tm thm1
 	val Pth = EXISTS(ep,x)(ASSUME P) and Qth = ASSUME Q
-	val thm2 = DISJ_CASES_UNION (ASSUME(mk_disj{disj1=P,disj2=Q})) Pth Qth 
-	val imp2 = DISCH otm (CHOOSE (x,ASSUME otm) thm2) 
+	val thm2 = DISJ_CASES_UNION (ASSUME(mk_disj{disj1=P,disj2=Q})) Pth Qth
+	val imp2 = DISCH otm (CHOOSE (x,ASSUME otm) thm2)
     in
 	GENL [f,Q] (IMP_ANTISYM_RULE imp1 imp2)
     end;
 
 val _ = save_thm("LEFT_OR_EXISTS_THM",LEFT_OR_EXISTS_THM);
-    
+
 
 (* ------------------------------------------------------------------------- *)
 (* RIGHT_OR_EXISTS_THM = |- P \/ (?x. Q x) = (?x. P \/ Q x)                  *)
@@ -1313,11 +1313,11 @@ val RIGHT_OR_EXISTS_THM =
 	val eq = mk_exists{Bvar=x,Body=Q}
 	val tm = mk_disj{disj1=P,disj2=eq}
 	val otm = mk_exists{Bvar=x,Body=mk_disj{disj1=P,disj2=Q}}
-	val t1 = DISJ1 (ASSUME P) Q and t2 = DISJ2 P (ASSUME Q) 
-	val th1 = EXISTS(otm,x) t1 and th2 = EXISTS(otm,x) t2 
-	val thm1 = DISJ_CASES (ASSUME tm) th1 (CHOOSE(x,ASSUME eq)th2) 
-	val imp1 = DISCH tm thm1 
-	val Qth = EXISTS(eq,x)(ASSUME Q) and Pth = ASSUME P 
+	val t1 = DISJ1 (ASSUME P) Q and t2 = DISJ2 P (ASSUME Q)
+	val th1 = EXISTS(otm,x) t1 and th2 = EXISTS(otm,x) t2
+	val thm1 = DISJ_CASES (ASSUME tm) th1 (CHOOSE(x,ASSUME eq)th2)
+	val imp1 = DISCH tm thm1
+	val Qth = EXISTS(eq,x)(ASSUME Q) and Pth = ASSUME P
 	val thm2 = DISJ_CASES_UNION (ASSUME(mk_disj{disj1=P,disj2=Q})) Pth Qth
 	val imp2 = DISCH otm (CHOOSE (x,ASSUME otm)  thm2)
     in
@@ -1325,38 +1325,38 @@ val RIGHT_OR_EXISTS_THM =
     end;
 
 val _ = save_thm("RIGHT_OR_EXISTS_THM",RIGHT_OR_EXISTS_THM);
-    
-	
+
+
 (* ------------------------------------------------------------------------- *)
 (* BOTH_EXISTS_AND_THM = |- !P Q. (?x. P /\ Q) = (?x. P) /\ (?x. Q)          *)
 (* ------------------------------------------------------------------------- *)
 
 val BOTH_EXISTS_AND_THM =
-    let	val x = (--`x:'a`--) 
-	val P = (--`P:bool`--) 
-	val Q = (--`Q:bool`--) 
-	val t = mk_conj{conj1=P,conj2=Q} 
+    let	val x = (--`x:'a`--)
+	val P = (--`P:bool`--)
+	val Q = (--`Q:bool`--)
+	val t = mk_conj{conj1=P,conj2=Q}
 	val exi = mk_exists{Bvar=x,Body=t}
 	val (t1,t2) = CONJ_PAIR (ASSUME t)
 	val t11 = EXISTS ((mk_exists{Bvar=x,Body=P}),x) t1
-	val t21 = EXISTS ((mk_exists{Bvar=x,Body=Q}),x) t2 
-	val imp1 = DISCH_ALL (CHOOSE (x, 
+	val t21 = EXISTS ((mk_exists{Bvar=x,Body=Q}),x) t2
+	val imp1 = DISCH_ALL (CHOOSE (x,
                     ASSUME (mk_exists{Bvar=x,Body=mk_conj{conj1=P,conj2=Q}}))
 		   (CONJ t11 t21))
-	val th21 = EXISTS (exi,x) (CONJ (ASSUME P) (ASSUME Q)) 
-	val th22 = CHOOSE(x,ASSUME(mk_exists{Bvar=x,Body=P})) th21 
-	val th23 = CHOOSE(x,ASSUME(mk_exists{Bvar=x,Body=Q})) th22 
+	val th21 = EXISTS (exi,x) (CONJ (ASSUME P) (ASSUME Q))
+	val th22 = CHOOSE(x,ASSUME(mk_exists{Bvar=x,Body=P})) th21
+	val th23 = CHOOSE(x,ASSUME(mk_exists{Bvar=x,Body=Q})) th22
 	val (u1,u2) =
 	    CONJ_PAIR (ASSUME (mk_conj{conj1=mk_exists{Bvar=x,Body=P},
 				       conj2=mk_exists{Bvar=x,Body=Q}}))
 	val th24 = PROVE_HYP u1 (PROVE_HYP u2 th23)
-	val imp2 = DISCH_ALL th24 
+	val imp2 = DISCH_ALL th24
     in
 	GENL [P,Q] (IMP_ANTISYM_RULE imp1 imp2)
     end;
 
 val _ = save_thm("BOTH_EXISTS_AND_THM",BOTH_EXISTS_AND_THM);
-    
+
 (* ------------------------------------------------------------------------- *)
 (* LEFT_EXISTS_AND_THM = |- !P Q. (?x. P x /\ Q) = (?x. P x) /\ Q            *)
 (* ------------------------------------------------------------------------- *)
@@ -1374,12 +1374,12 @@ val LEFT_EXISTS_AND_THM =
 	    DISCH_ALL
 		(CHOOSE
 		 (x, ASSUME (mk_exists{Bvar=x,Body=mk_conj{conj1=P,conj2=Q}}))
-		    (CONJ t11 t2)) 
-	val th21 = EXISTS (exi,x) (CONJ (ASSUME P) (ASSUME Q)) 
-	val th22 = CHOOSE(x,ASSUME(mk_exists{Bvar=x,Body=P})) th21 
+		    (CONJ t11 t2))
+	val th21 = EXISTS (exi,x) (CONJ (ASSUME P) (ASSUME Q))
+	val th22 = CHOOSE(x,ASSUME(mk_exists{Bvar=x,Body=P})) th21
 	val (u1,u2) = CONJ_PAIR(ASSUME
                        (mk_conj{conj1=mk_exists{Bvar=x,Body=P}, conj2=Q}))
-	val th23 = PROVE_HYP u1 (PROVE_HYP u2 th22) 
+	val th23 = PROVE_HYP u1 (PROVE_HYP u2 th22)
 	val imp2 = DISCH_ALL th23
     in
 	GENL [f,Q] (IMP_ANTISYM_RULE imp1 imp2)
@@ -1392,71 +1392,71 @@ val _ = save_thm("LEFT_EXISTS_AND_THM",LEFT_EXISTS_AND_THM);
 (* ------------------------------------------------------------------------- *)
 
 val RIGHT_EXISTS_AND_THM =
-    let	val x = (--`x:'a`--) 
-	val P = (--`P:bool`--) 
-	val g = (--`Q:'a->bool`--) 
-	val Q = mk_comb{Rator=g,Rand=x} 
-	val t = mk_conj{conj1=P,conj2=Q} 
-	val exi = mk_exists{Bvar=x,Body=t} 
-	val (t1,t2) = CONJ_PAIR (ASSUME t) 
-	val t21 = EXISTS ((mk_exists{Bvar=x,Body=Q}),x) t2 
+    let	val x = (--`x:'a`--)
+	val P = (--`P:bool`--)
+	val g = (--`Q:'a->bool`--)
+	val Q = mk_comb{Rator=g,Rand=x}
+	val t = mk_conj{conj1=P,conj2=Q}
+	val exi = mk_exists{Bvar=x,Body=t}
+	val (t1,t2) = CONJ_PAIR (ASSUME t)
+	val t21 = EXISTS ((mk_exists{Bvar=x,Body=Q}),x) t2
 	val imp1 =
 	    DISCH_ALL
 		(CHOOSE
 		 (x, ASSUME (mk_exists{Bvar=x,Body=mk_conj{conj1=P,conj2=Q}}))
-		 (CONJ t1 t21)) 
-	val th21 = EXISTS (exi,x) (CONJ (ASSUME P) (ASSUME Q)) 
+		 (CONJ t1 t21))
+	val th21 = EXISTS (exi,x) (CONJ (ASSUME P) (ASSUME Q))
 	val th22 = CHOOSE(x,ASSUME(mk_exists{Bvar=x,Body=Q})) th21
-	val (u1,u2) = CONJ_PAIR (ASSUME 
+	val (u1,u2) = CONJ_PAIR (ASSUME
                         (mk_conj{conj1=P, conj2=mk_exists{Bvar=x,Body=Q}}))
-	val th23 = PROVE_HYP u1 (PROVE_HYP u2 th22) 
-	val imp2 = DISCH_ALL th23 
+	val th23 = PROVE_HYP u1 (PROVE_HYP u2 th22)
+	val imp2 = DISCH_ALL th23
     in
 	GENL [P,g] (IMP_ANTISYM_RULE imp1 imp2)
     end;
 
 val _ = save_thm("RIGHT_EXISTS_AND_THM",RIGHT_EXISTS_AND_THM);
-    
+
 
 (* ------------------------------------------------------------------------- *)
 (* BOTH_FORALL_OR_THM = |- !P Q. (!x. P \/ Q) = (!x. P) \/ (!x. Q)           *)
 (* ------------------------------------------------------------------------- *)
 
 val BOTH_FORALL_OR_THM =
-  let val x = (--`x:'a`--) 
-      val P = (--`P:bool`--) 
-      val Q = (--`Q:bool`--) 
+  let val x = (--`x:'a`--)
+      val P = (--`P:bool`--)
+      val Q = (--`Q:bool`--)
       val imp11 = DISCH_ALL (SPEC x (ASSUME (mk_forall{Bvar=x,Body=P})))
-      val imp12 = DISCH_ALL (GEN x (ASSUME P)) 
-      val fath = IMP_ANTISYM_RULE imp11 imp12 
-      val th1 = REFL (mk_forall{Bvar=x, Body=mk_disj{disj1=P,disj2=Q}}) 
-      val th2 = CONV_RULE (RAND_CONV 
+      val imp12 = DISCH_ALL (GEN x (ASSUME P))
+      val fath = IMP_ANTISYM_RULE imp11 imp12
+      val th1 = REFL (mk_forall{Bvar=x, Body=mk_disj{disj1=P,disj2=Q}})
+      val th2 = CONV_RULE (RAND_CONV
                  (K (INST [P |-> mk_disj{disj1=P,disj2=Q}] fath))) th1
-      val th3 = CONV_RULE(RAND_CONV(RATOR_CONV(RAND_CONV(K(SYM fath))))) th2 
-      val th4 = CONV_RULE(RAND_CONV(RAND_CONV(K(SYM(INST[P|->Q] fath))))) th3 
+      val th3 = CONV_RULE(RAND_CONV(RATOR_CONV(RAND_CONV(K(SYM fath))))) th2
+      val th4 = CONV_RULE(RAND_CONV(RAND_CONV(K(SYM(INST[P|->Q] fath))))) th3
   in
-    GENL [P,Q] th4 
+    GENL [P,Q] th4
   end;
 
 val _ = save_thm("BOTH_FORALL_OR_THM",BOTH_FORALL_OR_THM);
-    
+
 (* ------------------------------------------------------------------------- *)
 (* LEFT_FORALL_OR_THM = |- !P Q. (!x. P x \/ Q) = (!x. P x) \/ Q             *)
 (* ------------------------------------------------------------------------- *)
 
 val LEFT_FORALL_OR_THM =
-  let val x = (--`x:'a`--) 
-      val f = (--`P:'a->bool`--) 
-      val P = mk_comb{Rator=f,Rand=x} 
-      val Q = (--`Q:bool`--) 
-      val tm = (mk_forall{Bvar=x,Body=mk_disj{disj1=P,disj2=Q}}) 
-      val thm1 = SPEC x (ASSUME tm) 
-      val thm2 = CONTR P (MP (ASSUME (mk_neg Q)) (ASSUME Q)) 
-      val thm3 = DISJ1 (GEN x (DISJ_CASES thm1 (ASSUME P) thm2)) Q 
+  let val x = (--`x:'a`--)
+      val f = (--`P:'a->bool`--)
+      val P = mk_comb{Rator=f,Rand=x}
+      val Q = (--`Q:bool`--)
+      val tm = (mk_forall{Bvar=x,Body=mk_disj{disj1=P,disj2=Q}})
+      val thm1 = SPEC x (ASSUME tm)
+      val thm2 = CONTR P (MP (ASSUME (mk_neg Q)) (ASSUME Q))
+      val thm3 = DISJ1 (GEN x (DISJ_CASES thm1 (ASSUME P) thm2)) Q
       val thm4 = DISJ2 (mk_forall{Bvar=x,Body=P}) (ASSUME Q)
-      val imp1 = DISCH tm (DISJ_CASES (SPEC Q EXCLUDED_MIDDLE) thm4 thm3) 
+      val imp1 = DISCH tm (DISJ_CASES (SPEC Q EXCLUDED_MIDDLE) thm4 thm3)
       val thm5 = SPEC x (ASSUME (mk_forall{Bvar=x,Body=P}))
-      val thm6 = ASSUME Q 
+      val thm6 = ASSUME Q
       val imp2 = DISCH_ALL (GEN x (DISJ_CASES_UNION
                   (ASSUME(mk_disj{disj1=mk_forall{Bvar=x,Body=P}, disj2=Q}))
                    thm5 thm6))
@@ -1465,23 +1465,23 @@ val LEFT_FORALL_OR_THM =
   end;
 
 val _ = save_thm("LEFT_FORALL_OR_THM",LEFT_FORALL_OR_THM);
-    
+
 (* ------------------------------------------------------------------------- *)
 (* RIGHT_FORALL_OR_THM = |- !P Q. (!x. P \/ Q x) = P \/ (!x. Q x)            *)
 (* ------------------------------------------------------------------------- *)
 
 val RIGHT_FORALL_OR_THM =
-    let	val x = (--`x:'a`--) 
-	val P = (--`P:bool`--) 
-	val g = (--`Q:'a->bool`--) 
-	val Q = mk_comb{Rator=g,Rand=x} 
-	val tm = (mk_forall{Bvar=x,Body=mk_disj{disj1=P,disj2=Q}}) 
-	val thm1 = SPEC x (ASSUME tm) 
-	val thm2 = CONTR Q (MP (ASSUME (mk_neg P)) (ASSUME P)) 
-	val thm3 = DISJ2 P (GEN x (DISJ_CASES thm1 thm2 (ASSUME Q))) 
+    let	val x = (--`x:'a`--)
+	val P = (--`P:bool`--)
+	val g = (--`Q:'a->bool`--)
+	val Q = mk_comb{Rator=g,Rand=x}
+	val tm = (mk_forall{Bvar=x,Body=mk_disj{disj1=P,disj2=Q}})
+	val thm1 = SPEC x (ASSUME tm)
+	val thm2 = CONTR Q (MP (ASSUME (mk_neg P)) (ASSUME P))
+	val thm3 = DISJ2 P (GEN x (DISJ_CASES thm1 thm2 (ASSUME Q)))
 	val thm4 = DISJ1 (ASSUME P) (mk_forall{Bvar=x,Body=Q})
-	val imp1 = DISCH tm (DISJ_CASES (SPEC P EXCLUDED_MIDDLE) thm4 thm3) 
-	val thm5 = ASSUME P 
+	val imp1 = DISCH tm (DISJ_CASES (SPEC P EXCLUDED_MIDDLE) thm4 thm3)
+	val thm5 = ASSUME P
 	val thm6 = SPEC x (ASSUME (mk_forall{Bvar=x,Body=Q}))
 	val imp2 = DISCH_ALL (GEN x (DISJ_CASES_UNION
                    (ASSUME (mk_disj{disj1=P, disj2=mk_forall{Bvar=x,Body=Q}}))
@@ -1491,7 +1491,7 @@ val RIGHT_FORALL_OR_THM =
     end;
 
 val _ = save_thm("RIGHT_FORALL_OR_THM",RIGHT_FORALL_OR_THM);
-    
+
 
 (* ------------------------------------------------------------------------- *)
 (* BOTH_FORALL_IMP_THM = |- (!x. P ==> Q) = ((?x.P) ==> (!x.Q))              *)
@@ -1499,136 +1499,136 @@ val _ = save_thm("RIGHT_FORALL_OR_THM",RIGHT_FORALL_OR_THM);
 
 val BOTH_FORALL_IMP_THM =
     let val x = (--`x:'a`--)
-	val P = (--`P:bool`--) 
-	val Q = (--`Q:bool`--) 
+	val P = (--`P:bool`--)
+	val Q = (--`Q:bool`--)
 	val tm = mk_forall{Bvar=x, Body=mk_imp{ant=P,conseq= Q}}
-	val asm = mk_exists{Bvar=x,Body=P} 
-	val th1 = GEN x (CHOOSE(x,ASSUME asm)(UNDISCH(SPEC x (ASSUME tm)))) 
-	val imp1 = DISCH tm (DISCH asm th1) 
-	val cncl = rand(concl imp1) 
-	val th2 = SPEC x (MP (ASSUME cncl) (EXISTS (asm,x) (ASSUME P))) 
-	val imp2 = DISCH cncl (GEN x (DISCH P th2)) 
+	val asm = mk_exists{Bvar=x,Body=P}
+	val th1 = GEN x (CHOOSE(x,ASSUME asm)(UNDISCH(SPEC x (ASSUME tm))))
+	val imp1 = DISCH tm (DISCH asm th1)
+	val cncl = rand(concl imp1)
+	val th2 = SPEC x (MP (ASSUME cncl) (EXISTS (asm,x) (ASSUME P)))
+	val imp2 = DISCH cncl (GEN x (DISCH P th2))
     in
-	GENL [P,Q] (IMP_ANTISYM_RULE imp1 imp2) 
+	GENL [P,Q] (IMP_ANTISYM_RULE imp1 imp2)
     end;
 
 val _ = save_thm("BOTH_FORALL_IMP_THM",BOTH_FORALL_IMP_THM);
-    
+
 
 (* ------------------------------------------------------------------------- *)
 (* LEFT_FORALL_IMP_THM = |- (!x. P[x]==>Q) = ((?x.P[x]) ==> Q)               *)
 (* ------------------------------------------------------------------------- *)
 
 val LEFT_FORALL_IMP_THM =
-    let	val x = (--`x:'a`--) 
-	val f = (--`P:'a->bool`--) 
-	val P = mk_comb{Rator=f,Rand=x} 
-	val Q = (--`Q:bool`--) 
-	val tm = mk_forall{Bvar=x, Body= mk_imp {ant=P,conseq=Q}} 
-	val asm = mk_exists{Bvar=x,Body=P} 
-	val th1 = CHOOSE(x,ASSUME asm)(UNDISCH(SPEC x (ASSUME tm))) 
-	val imp1 = DISCH tm (DISCH asm th1) 
-	val cncl = rand(concl imp1) 
-	val th2 = MP (ASSUME cncl) (EXISTS (asm,x) (ASSUME P)) 
-	val imp2 = DISCH cncl (GEN x (DISCH P th2)) 
+    let	val x = (--`x:'a`--)
+	val f = (--`P:'a->bool`--)
+	val P = mk_comb{Rator=f,Rand=x}
+	val Q = (--`Q:bool`--)
+	val tm = mk_forall{Bvar=x, Body= mk_imp {ant=P,conseq=Q}}
+	val asm = mk_exists{Bvar=x,Body=P}
+	val th1 = CHOOSE(x,ASSUME asm)(UNDISCH(SPEC x (ASSUME tm)))
+	val imp1 = DISCH tm (DISCH asm th1)
+	val cncl = rand(concl imp1)
+	val th2 = MP (ASSUME cncl) (EXISTS (asm,x) (ASSUME P))
+	val imp2 = DISCH cncl (GEN x (DISCH P th2))
     in
-	GENL [f,Q] (IMP_ANTISYM_RULE imp1 imp2) 
+	GENL [f,Q] (IMP_ANTISYM_RULE imp1 imp2)
     end;
 
 val _ = save_thm("LEFT_FORALL_IMP_THM",LEFT_FORALL_IMP_THM);
-    
+
 (* ------------------------------------------------------------------------- *)
 (* RIGHT_FORALL_IMP_THM = |- (!x. P==>Q[x]) = (P ==> (!x.Q[x]))              *)
 (* ------------------------------------------------------------------------- *)
 
 val RIGHT_FORALL_IMP_THM =
-    let val x = (--`x:'a`--) 
-	val P = (--`P:bool`--) 
-	val g = (--`Q:'a->bool`--) 
-	val Q = mk_comb{Rator=g,Rand=x} 
-	val tm = mk_forall{Bvar=x, Body=mk_imp{ant=P,conseq=Q}} 
-	val imp1 = DISCH P(GEN x(UNDISCH(SPEC x(ASSUME tm)))) 
-	val cncl = concl imp1 
-	val imp2 = GEN x (DISCH P(SPEC x(UNDISCH (ASSUME cncl)))) 
+    let val x = (--`x:'a`--)
+	val P = (--`P:bool`--)
+	val g = (--`Q:'a->bool`--)
+	val Q = mk_comb{Rator=g,Rand=x}
+	val tm = mk_forall{Bvar=x, Body=mk_imp{ant=P,conseq=Q}}
+	val imp1 = DISCH P(GEN x(UNDISCH(SPEC x(ASSUME tm))))
+	val cncl = concl imp1
+	val imp2 = GEN x (DISCH P(SPEC x(UNDISCH (ASSUME cncl))))
     in
-	GENL [P,g] (IMP_ANTISYM_RULE (DISCH tm imp1) (DISCH cncl imp2)) 
+	GENL [P,g] (IMP_ANTISYM_RULE (DISCH tm imp1) (DISCH cncl imp2))
     end;
 
 val _ = save_thm("RIGHT_FORALL_IMP_THM",RIGHT_FORALL_IMP_THM);
-    
+
 
 (* ------------------------------------------------------------------------- *)
 (* BOTH_EXISTS_IMP_THM = |- (?x. P ==> Q) = ((!x.P) ==> (?x.Q))              *)
 (* ------------------------------------------------------------------------- *)
 
 val BOTH_EXISTS_IMP_THM =
-    let val x = (--`x:'a`--) 
-	val P = (--`P:bool`--) 
-	val Q = (--`Q:bool`--) 
-	val tm = mk_exists{Bvar=x,Body=mk_imp{ant=P,conseq=Q}} 
-	val eQ = mk_exists{Bvar=x,Body=Q} 
-	val aP = mk_forall{Bvar=x,Body=P} 
-	val thm1 = EXISTS(eQ,x)(UNDISCH(ASSUME(mk_imp{ant=P,conseq=Q}))) 
-	val thm2 = DISCH aP (PROVE_HYP (SPEC x (ASSUME aP)) thm1) 
-	val imp1 = DISCH tm (CHOOSE(x,ASSUME tm) thm2) 
+    let val x = (--`x:'a`--)
+	val P = (--`P:bool`--)
+	val Q = (--`Q:bool`--)
+	val tm = mk_exists{Bvar=x,Body=mk_imp{ant=P,conseq=Q}}
+	val eQ = mk_exists{Bvar=x,Body=Q}
+	val aP = mk_forall{Bvar=x,Body=P}
+	val thm1 = EXISTS(eQ,x)(UNDISCH(ASSUME(mk_imp{ant=P,conseq=Q})))
+	val thm2 = DISCH aP (PROVE_HYP (SPEC x (ASSUME aP)) thm1)
+	val imp1 = DISCH tm (CHOOSE(x,ASSUME tm) thm2)
 	val thm2 = CHOOSE(x,UNDISCH (ASSUME (rand(concl imp1)))) (ASSUME Q)
-	val thm3 = DISCH P (PROVE_HYP (GEN x (ASSUME P)) thm2) 
+	val thm3 = DISCH P (PROVE_HYP (GEN x (ASSUME P)) thm2)
 	val imp2 = DISCH (rand(concl imp1)) (EXISTS(tm,x) thm3)
     in
 	GENL [P,Q] (IMP_ANTISYM_RULE imp1 imp2)
     end;
 
 val _ = save_thm("BOTH_EXISTS_IMP_THM",BOTH_EXISTS_IMP_THM);
-    
+
 
 (* ------------------------------------------------------------------------- *)
 (* LEFT_EXISTS_IMP_THM = |- (?x. P[x] ==> Q) = ((!x.P[x]) ==> Q)             *)
 (* ------------------------------------------------------------------------- *)
 
 val LEFT_EXISTS_IMP_THM =
-    let	val x = (--`x:'a`--) 
-	val f = (--`P:'a->bool`--) 
-	val P = mk_comb{Rator=f,Rand=x} 
-	val Q = (--`Q:bool`--) 
-	val tm = mk_exists{Bvar=x, Body= mk_imp{ant=P,conseq=Q}} 
-	val allp = mk_forall{Bvar=x,Body=P} 
-	val th1 = SPEC x (ASSUME allp) 
-	val thm1 = MP (ASSUME(mk_imp{ant=P,conseq=Q})) th1 
-	val imp1 = DISCH tm (CHOOSE(x,ASSUME tm)(DISCH allp thm1)) 
-	val otm = rand(concl imp1) 
-	val thm2 = EXISTS(tm,x)(DISCH P (UNDISCH(ASSUME otm))) 
-	val nex =  mk_exists{Bvar=x,Body=mk_neg P} 
-	val asm1 = EXISTS (nex, x) (ASSUME (mk_neg P)) 
-	val th2 = CCONTR P (MP (ASSUME (mk_neg nex)) asm1) 
-	val th3 = CCONTR nex (MP (ASSUME (mk_neg allp)) (GEN x th2)) 
-	val thm4 = DISCH P (CONTR Q (UNDISCH (ASSUME (mk_neg P)))) 
-	val thm5 = CHOOSE(x,th3)(EXISTS(tm,x)thm4) 
-	val thm6 = DISJ_CASES (SPEC allp EXCLUDED_MIDDLE) thm2 thm5 
-	val imp2 = DISCH otm thm6 
+    let	val x = (--`x:'a`--)
+	val f = (--`P:'a->bool`--)
+	val P = mk_comb{Rator=f,Rand=x}
+	val Q = (--`Q:bool`--)
+	val tm = mk_exists{Bvar=x, Body= mk_imp{ant=P,conseq=Q}}
+	val allp = mk_forall{Bvar=x,Body=P}
+	val th1 = SPEC x (ASSUME allp)
+	val thm1 = MP (ASSUME(mk_imp{ant=P,conseq=Q})) th1
+	val imp1 = DISCH tm (CHOOSE(x,ASSUME tm)(DISCH allp thm1))
+	val otm = rand(concl imp1)
+	val thm2 = EXISTS(tm,x)(DISCH P (UNDISCH(ASSUME otm)))
+	val nex =  mk_exists{Bvar=x,Body=mk_neg P}
+	val asm1 = EXISTS (nex, x) (ASSUME (mk_neg P))
+	val th2 = CCONTR P (MP (ASSUME (mk_neg nex)) asm1)
+	val th3 = CCONTR nex (MP (ASSUME (mk_neg allp)) (GEN x th2))
+	val thm4 = DISCH P (CONTR Q (UNDISCH (ASSUME (mk_neg P))))
+	val thm5 = CHOOSE(x,th3)(EXISTS(tm,x)thm4)
+	val thm6 = DISJ_CASES (SPEC allp EXCLUDED_MIDDLE) thm2 thm5
+	val imp2 = DISCH otm thm6
     in
-	GENL [f, Q] (IMP_ANTISYM_RULE imp1 imp2) 
+	GENL [f, Q] (IMP_ANTISYM_RULE imp1 imp2)
     end;
 
 val _ = save_thm("LEFT_EXISTS_IMP_THM",LEFT_EXISTS_IMP_THM);
-    
+
 
 (* ------------------------------------------------------------------------- *)
 (* RIGHT_EXISTS_IMP_THM = |- (?x. P ==> Q[x]) = (P ==> (?x.Q[x]))            *)
 (* ------------------------------------------------------------------------- *)
 
 val RIGHT_EXISTS_IMP_THM =
-    let	val x = (--`x:'a`--) 
-	val P = (--`P:bool`--) 
-	val g = (--`Q:'a->bool`--) 
-	val Q = mk_comb{Rator=g,Rand=x} 
-	val tm = mk_exists{Bvar=x,Body=mk_imp{ant=P,conseq=Q}} 
+    let	val x = (--`x:'a`--)
+	val P = (--`P:bool`--)
+	val g = (--`Q:'a->bool`--)
+	val Q = mk_comb{Rator=g,Rand=x}
+	val tm = mk_exists{Bvar=x,Body=mk_imp{ant=P,conseq=Q}}
 	val thm1 = EXISTS (mk_exists{Bvar=x,Body=Q},x)
 	                   (UNDISCH(ASSUME(mk_imp{ant=P,conseq=Q})))
-	val imp1 = DISCH tm (CHOOSE(x,ASSUME tm) (DISCH P thm1)) 
-	val thm2 = UNDISCH (ASSUME (rand(concl imp1))) 
-	val thm3 = CHOOSE (x,thm2) (EXISTS (tm,x) (DISCH P (ASSUME Q))) 
-	val thm4 = EXISTS(tm,x)(DISCH P(CONTR Q(UNDISCH(ASSUME(mk_neg P))))) 
-	val thm5 = DISJ_CASES (SPEC P EXCLUDED_MIDDLE) thm3 thm4 
+	val imp1 = DISCH tm (CHOOSE(x,ASSUME tm) (DISCH P thm1))
+	val thm2 = UNDISCH (ASSUME (rand(concl imp1)))
+	val thm3 = CHOOSE (x,thm2) (EXISTS (tm,x) (DISCH P (ASSUME Q)))
+	val thm4 = EXISTS(tm,x)(DISCH P(CONTR Q(UNDISCH(ASSUME(mk_neg P)))))
+	val thm5 = DISJ_CASES (SPEC P EXCLUDED_MIDDLE) thm3 thm4
 	val imp2 = DISCH(rand(concl imp1)) thm5
     in
 	GENL [P,g] (IMP_ANTISYM_RULE imp1 imp2)
@@ -1641,18 +1641,18 @@ val _ = save_thm("RIGHT_EXISTS_IMP_THM",RIGHT_EXISTS_IMP_THM);
 (* [TFM 90.06.28]                                                        *)
 (* --------------------------------------------------------------------- *)
 
-val OR_IMP_THM = 
- let val t1 = (--`A:bool`--) and t2 = (--`B:bool`--) 
-     val asm1 = ASSUME (--`^t1 = (^t2 \/ ^t1)`--) 
+val OR_IMP_THM =
+ let val t1 = (--`A:bool`--) and t2 = (--`B:bool`--)
+     val asm1 = ASSUME (--`^t1 = (^t2 \/ ^t1)`--)
      and asm2 = EQT_INTRO(ASSUME t2)
-     val th1 = SUBST [t2 |-> asm2] (concl asm1) asm1 
-     val th2 = TRANS th1 (CONJUNCT1 (SPEC t1 OR_CLAUSES)) 
-     val imp1 = DISCH (concl asm1) (DISCH t2 (EQT_ELIM th2)) 
-     val asm3 = ASSUME (--`^t2 ==> ^t1`--) 
-     and asm4 = ASSUME (--`^t2 \/ ^t1`--) 
-     val th3 = DISJ_CASES asm4 (MP asm3 (ASSUME t2)) (ASSUME t1) 
-     val th4 = DISCH (concl asm4) th3 
-     and th5 = DISCH t1 (DISJ2 t2 (ASSUME t1)) 
+     val th1 = SUBST [t2 |-> asm2] (concl asm1) asm1
+     val th2 = TRANS th1 (CONJUNCT1 (SPEC t1 OR_CLAUSES))
+     val imp1 = DISCH (concl asm1) (DISCH t2 (EQT_ELIM th2))
+     val asm3 = ASSUME (--`^t2 ==> ^t1`--)
+     and asm4 = ASSUME (--`^t2 \/ ^t1`--)
+     val th3 = DISJ_CASES asm4 (MP asm3 (ASSUME t2)) (ASSUME t1)
+     val th4 = DISCH (concl asm4) th3
+     and th5 = DISCH t1 (DISJ2 t2 (ASSUME t1))
      val imp2 = DISCH (--`^t2 ==> ^t1`--) (IMP_ANTISYM_RULE th5 th4)
   in
    GEN t1 (GEN t2 (IMP_ANTISYM_RULE imp1 imp2))
@@ -1665,20 +1665,20 @@ val _ = save_thm("OR_IMP_THM",OR_IMP_THM);
 (* [TFM 90.07.09]                                                        *)
 (* --------------------------------------------------------------------- *)
 
-val NOT_IMP = 
-let val t1 = (--`A:bool`--) and t2 = (--`B:bool`--) 
-    val asm1 = ASSUME (--`~(^t1 ==> ^t2)`--) 
-    val thm1 = SUBST [t1 |-> EQF_INTRO (ASSUME (mk_neg t1))] (concl asm1) asm1 
+val NOT_IMP =
+let val t1 = (--`A:bool`--) and t2 = (--`B:bool`--)
+    val asm1 = ASSUME (--`~(^t1 ==> ^t2)`--)
+    val thm1 = SUBST [t1 |-> EQF_INTRO (ASSUME (mk_neg t1))] (concl asm1) asm1
     val thm2 = CCONTR t1 (MP thm1 (DISCH(--`F`--)(CONTR t2 (ASSUME(--`F`--)))))
-    val thm3 = SUBST [t2 |-> EQT_INTRO (ASSUME t2)] (concl asm1) asm1 
-    val thm4 = NOT_INTRO(DISCH t2 (MP thm3 (DISCH t1 (ADD_ASSUM t1 TRUTH)))) 
-    val imp1 = DISCH (concl asm1) (CONJ thm2 thm4) 
-    val conj =  ASSUME (--`^t1 /\ ~^t2`--) 
-    val (asm2,asm3) = (CONJUNCT1 conj, CONJUNCT2 conj) 
-    val asm4 = ASSUME (--`^t1 ==> ^t2`--) 
-    val thm5 = MP (SUBST [t2 |-> EQF_INTRO asm3] (concl asm4) asm4) asm2 
-    val imp2 = DISCH (--`^t1 /\ ~ ^t2`--) 
-                     (NOT_INTRO(DISCH (--`^t1 ==> ^t2`--) thm5)) 
+    val thm3 = SUBST [t2 |-> EQT_INTRO (ASSUME t2)] (concl asm1) asm1
+    val thm4 = NOT_INTRO(DISCH t2 (MP thm3 (DISCH t1 (ADD_ASSUM t1 TRUTH))))
+    val imp1 = DISCH (concl asm1) (CONJ thm2 thm4)
+    val conj =  ASSUME (--`^t1 /\ ~^t2`--)
+    val (asm2,asm3) = (CONJUNCT1 conj, CONJUNCT2 conj)
+    val asm4 = ASSUME (--`^t1 ==> ^t2`--)
+    val thm5 = MP (SUBST [t2 |-> EQF_INTRO asm3] (concl asm4) asm4) asm2
+    val imp2 = DISCH (--`^t1 /\ ~ ^t2`--)
+                     (NOT_INTRO(DISCH (--`^t1 ==> ^t2`--) thm5))
  in
     GEN t1 (GEN t2 (IMP_ANTISYM_RULE imp1 imp2))
  end;
@@ -1691,20 +1691,20 @@ val _ = save_thm("NOT_IMP", NOT_IMP);
 fun mk_disj(x,y) = Dsyntax.mk_disj{disj1=x,disj2=y}
 fun mk_conj(x,y) = Dsyntax.mk_conj{conj1=x,conj2=y};
 
-val DISJ_ASSOC = 
+val DISJ_ASSOC =
 let val t1 = (--`A:bool`--) and t2 = (--`B:bool`--) and t3 = (--`C:bool`--)
     val at1 = DISJ1 (DISJ1 (ASSUME t1) t2) t3 and
         at2 = DISJ1 (DISJ2 t1 (ASSUME t2)) t3 and
-        at3 = DISJ2 (mk_disj(t1,t2)) (ASSUME t3) 
-    val thm = DISJ_CASES (ASSUME (mk_disj(t2,t3))) at2 at3 
-    val thm1 = DISJ_CASES (ASSUME (mk_disj(t1,mk_disj(t2,t3)))) at1 thm 
+        at3 = DISJ2 (mk_disj(t1,t2)) (ASSUME t3)
+    val thm = DISJ_CASES (ASSUME (mk_disj(t2,t3))) at2 at3
+    val thm1 = DISJ_CASES (ASSUME (mk_disj(t1,mk_disj(t2,t3)))) at1 thm
     val at1 = DISJ1 (ASSUME t1) (mk_disj(t2,t3)) and
         at2 = DISJ2 t1 (DISJ1 (ASSUME t2) t3) and
-        at3 = DISJ2 t1 (DISJ2 t2 (ASSUME t3)) 
-    val thm = DISJ_CASES (ASSUME (mk_disj(t1,t2))) at1 at2 
-    val thm2 = DISJ_CASES (ASSUME (mk_disj(mk_disj(t1,t2),t3))) thm at3 
+        at3 = DISJ2 t1 (DISJ2 t2 (ASSUME t3))
+    val thm = DISJ_CASES (ASSUME (mk_disj(t1,t2))) at1 at2
+    val thm2 = DISJ_CASES (ASSUME (mk_disj(mk_disj(t1,t2),t3))) thm at3
     val imp1 = DISCH (mk_disj(t1,mk_disj(t2,t3))) thm1 and
-        imp2 = DISCH (mk_disj(mk_disj(t1,t2),t3)) thm2 
+        imp2 = DISCH (mk_disj(mk_disj(t1,t2),t3)) thm2
  in
    GENL [t1,t2,t3] (IMP_ANTISYM_RULE imp1 imp2)
  end;
@@ -1716,13 +1716,13 @@ val _ = save_thm("DISJ_ASSOC", DISJ_ASSOC);
 (* --------------------------------------------------------------------- *)
 
 val DISJ_SYM =
-let val t1   = (--`A:bool`--) and t2 = (--`B:bool`--) 
-    val th1  = DISJ1 (ASSUME t1) t2 and th2 = DISJ2 t1 (ASSUME t2) 
-    val thm1 = DISJ_CASES (ASSUME(mk_disj(t2,t1))) th2 th1 
-    val th1  = DISJ1 (ASSUME t2) t1 and th2 = DISJ2 t2 (ASSUME t1) 
-    val thm2 = DISJ_CASES (ASSUME(mk_disj(t1,t2))) th2 th1 
+let val t1   = (--`A:bool`--) and t2 = (--`B:bool`--)
+    val th1  = DISJ1 (ASSUME t1) t2 and th2 = DISJ2 t1 (ASSUME t2)
+    val thm1 = DISJ_CASES (ASSUME(mk_disj(t2,t1))) th2 th1
+    val th1  = DISJ1 (ASSUME t2) t1 and th2 = DISJ2 t2 (ASSUME t1)
+    val thm2 = DISJ_CASES (ASSUME(mk_disj(t1,t2))) th2 th1
     val imp1 = DISCH (mk_disj(t2,t1)) thm1 and
-        imp2 = DISCH (mk_disj(t1,t2)) thm2 
+        imp2 = DISCH (mk_disj(t1,t2)) thm2
  in
    GENL [t1,t2] (IMP_ANTISYM_RULE imp2 imp1)
  end;
@@ -1734,49 +1734,49 @@ val _ = save_thm("DISJ_SYM", DISJ_SYM);
 (*  |- !A B. (~(t1 /\ t2) = ~t1 \/ ~t2) /\ (~(t1 \/ t2) = ~t1 /\ ~t2)    *)
 (* --------------------------------------------------------------------- *)
 
-val DE_MORGAN_THM = 
-let val t1 = (--`A:bool`--) and t2 = (--`B:bool`--) 
-    val thm1 = 
-      let val asm1 = ASSUME (--`~(^t1 /\ ^t2)`--) 
-          val cnj = MP asm1 (CONJ (ASSUME t1) (ASSUME t2)) 
-          val imp1 = 
-            let val case1 = DISJ2 (--`~^t1`--) (NOT_INTRO(DISCH t2 cnj)) 
-                val case2 = DISJ1 (ASSUME (--`~ ^t1`--)) (--`~ ^t2`--) 
+val DE_MORGAN_THM =
+let val t1 = (--`A:bool`--) and t2 = (--`B:bool`--)
+    val thm1 =
+      let val asm1 = ASSUME (--`~(^t1 /\ ^t2)`--)
+          val cnj = MP asm1 (CONJ (ASSUME t1) (ASSUME t2))
+          val imp1 =
+            let val case1 = DISJ2 (--`~^t1`--) (NOT_INTRO(DISCH t2 cnj))
+                val case2 = DISJ1 (ASSUME (--`~ ^t1`--)) (--`~ ^t2`--)
             in
-              DISJ_CASES (SPEC t1 EXCLUDED_MIDDLE) case1 case2 
+              DISJ_CASES (SPEC t1 EXCLUDED_MIDDLE) case1 case2
             end
-          val th1 = MP (ASSUME (--`~^t1`--)) 
+          val th1 = MP (ASSUME (--`~^t1`--))
                        (CONJUNCT1 (ASSUME (--`^t1 /\ ^t2`--)))
-          val th2 = MP (ASSUME (--`~^t2`--)) 
-                   (CONJUNCT2 (ASSUME (--`^t1 /\ ^t2`--))) 
-          val imp2 = 
-            let val fth = DISJ_CASES (ASSUME (--`~^t1 \/ ~^t2`--)) th1 th2 
+          val th2 = MP (ASSUME (--`~^t2`--))
+                   (CONJUNCT2 (ASSUME (--`^t1 /\ ^t2`--)))
+          val imp2 =
+            let val fth = DISJ_CASES (ASSUME (--`~^t1 \/ ~^t2`--)) th1 th2
             in
-              DISCH (--`~^t1 \/ ~^t2`--) 
+              DISCH (--`~^t1 \/ ~^t2`--)
                     (NOT_INTRO(DISCH (--`^t1 /\ ^t2`--) fth))
             end
       in
         IMP_ANTISYM_RULE (DISCH (--`~(^t1 /\ ^t2)`--) imp1) imp2
       end
-    val thm2 = 
-      let val asm1 = ASSUME (--`~(^t1 \/ ^t2)`--) 
-          val imp1 = 
+    val thm2 =
+      let val asm1 = ASSUME (--`~(^t1 \/ ^t2)`--)
+          val imp1 =
             let val th1 = NOT_INTRO (DISCH t1(MP asm1 (DISJ1 (ASSUME t1) t2)))
                 val th2 = NOT_INTRO (DISCH t2 (MP asm1 (DISJ2 t1 (ASSUME t2))))
             in
-              DISCH (--`~(^t1 \/ ^t2)`--) (CONJ th1 th2) 
+              DISCH (--`~(^t1 \/ ^t2)`--) (CONJ th1 th2)
             end
-          val imp2 = 
-            let val asm = ASSUME (--`^t1 \/ ^t2`--) 
+          val imp2 =
+            let val asm = ASSUME (--`^t1 \/ ^t2`--)
                 val a1 = CONJUNCT1(ASSUME (--`~^t1 /\ ~^t2`--)) and
-                    a2 = CONJUNCT2(ASSUME (--`~^t1 /\ ~^t2`--)) 
+                    a2 = CONJUNCT2(ASSUME (--`~^t1 /\ ~^t2`--))
                val fth = DISJ_CASES asm (UNDISCH a1) (UNDISCH a2)
             in
-                DISCH (--`~^t1 /\ ~^t2`--) 
+                DISCH (--`~^t1 /\ ~^t2`--)
                       (NOT_INTRO(DISCH (--`^t1 \/ ^t2`--) fth))
             end
       in
-        IMP_ANTISYM_RULE imp1 imp2 
+        IMP_ANTISYM_RULE imp1 imp2
       end
  in
     GEN t1 (GEN t2 (CONJ thm1 thm2))
@@ -1796,7 +1796,7 @@ val _ = save_thm("DE_MORGAN_THM", DE_MORGAN_THM);
 (* RIGHT_OR_OVER_AND  |- !A B C. B /\ C \/ A = (B \/ A) /\ (C \/ A)         *)
 (* -------------------------------------------------------------------------*)
 
-val LEFT_AND_OVER_OR = 
+val LEFT_AND_OVER_OR =
     let val t1 = --`A:bool`--
         and t2 = --`B:bool`--
         and t3 = --`C:bool`--
@@ -1815,7 +1815,7 @@ val LEFT_AND_OVER_OR =
 
 val _ = save_thm("LEFT_AND_OVER_OR", LEFT_AND_OVER_OR);
 
-val RIGHT_AND_OVER_OR = 
+val RIGHT_AND_OVER_OR =
    let val t1 = --`A:bool`--
        and t2 = --`B:bool`--
        and t3 = --`C:bool`--
@@ -1831,10 +1831,10 @@ val RIGHT_AND_OVER_OR =
    in
      GEN t1 (GEN t2 (GEN t3 (IMP_ANTISYM_RULE imp1 imp2)))
    end;
-  
+
 val _ = save_thm("RIGHT_AND_OVER_OR", RIGHT_AND_OVER_OR);
 
-val LEFT_OR_OVER_AND = 
+val LEFT_OR_OVER_AND =
    let val t1 = --`A:bool`--
        and t2 = --`B:bool`--
        and t3 = --`C:bool`--
@@ -1855,7 +1855,7 @@ val LEFT_OR_OVER_AND =
 
 val _ = save_thm("LEFT_OR_OVER_AND", LEFT_OR_OVER_AND);
 
-val RIGHT_OR_OVER_AND = 
+val RIGHT_OR_OVER_AND =
    let val t1 = --`A:bool`--
        and t2 = --`B:bool`--
        and t3 = --`C:bool`--
@@ -1865,7 +1865,7 @@ val RIGHT_OR_OVER_AND =
        val th5 = CONJ (DISJ1 th3 t1) (DISJ1 th4 t1)
        val imp1 = DISCH (concl th1) (DISJ_CASES th1 th5 th2)
        val (th1,th2) = CONJ_PAIR (ASSUME (rand(concl imp1)))
-       val th3 = DISJ2 (mk_conj(t2,t3)) (ASSUME t1) 
+       val th3 = DISJ2 (mk_conj(t2,t3)) (ASSUME t1)
        val (th4,th5) = CONJ_PAIR (ASSUME (mk_conj(t2,t3)))
        val th4 = DISJ1 (CONJ (ASSUME t2) (ASSUME t3)) t1
        val th5 = DISJ_CASES th2 (DISJ_CASES th1 th4 th3) th3
@@ -1880,13 +1880,13 @@ val _ = save_thm("RIGHT_OR_OVER_AND", RIGHT_OR_OVER_AND);
 (*---------------------------------------------------------------------------*
  * IMP_DISJ_THM = |- !A B. A ==> B = ~A \/ B                                 *
  *---------------------------------------------------------------------------*)
-val IMP_DISJ_THM = 
+val IMP_DISJ_THM =
 let val A = --`A:bool`--
     val B = --`B:bool`--
     val th1 = ASSUME (Term`A ==> B`)
     val th2 = ASSUME A
     val th3 = MP th1 th2
-    val th4 = DISJ2 (Term`~A`) th3 
+    val th4 = DISJ2 (Term`~A`) th3
     val th5 = ASSUME (Term`~A`);
     val th6 = ADD_ASSUM (Term`A ==> B`) th5
     val th7 = DISJ1 th6 B
@@ -1902,11 +1902,43 @@ let val A = --`A:bool`--
     val th16 = SUBST [A |-> th15] A th14
     val th17 = DISCH A th16
     val th18 = DISCH (concl th11) th17
- in 
+ in
    GENL [A,B] (IMP_ANTISYM_RULE (DISCH (hd(hyp th9)) th9) th18)
  end;
 
 val _ = save_thm ("IMP_DISJ_THM", IMP_DISJ_THM);
+
+(*----------------------------------------------------------------------*)
+(* DISJ_IMP_THM = |- !P Q R. P \/ Q ==> R = (P ==> R) /\ (Q ==> R)      *)
+(*                                                         MN 99.05.06  *)
+(*----------------------------------------------------------------------*)
+
+val DISJ_IMP_THM = let
+  val P = --`P:bool`--
+  val Q = --`Q:bool`--
+  val R = --`R:bool`--
+  val lhs = --`P \/ Q ==> R`--
+  val rhs = --`(P ==> R) /\ (Q ==> R)`--
+  val ass_lhs = ASSUME lhs
+  val ass_P = ASSUME P
+  val ass_Q = ASSUME Q
+  val p_imp_r = DISCH P (MP ass_lhs (DISJ1 ass_P Q))
+  val q_imp_r = DISCH Q (MP ass_lhs (DISJ2 P ass_Q))
+  val lr_imp = DISCH lhs (CONJ p_imp_r q_imp_r)
+  (* half way there! *)
+  val ass_rhs = ASSUME rhs
+  val porq = (--`P \/ Q`--)
+  val ass_porq = ASSUME porq
+  val my_and1 = SPECL [(--`P ==> R`--), (--`Q ==> R`--)] AND1_THM
+  val p_imp_r = MP my_and1 ass_rhs
+  val r_from_p = MP p_imp_r ass_P
+  val my_and2 = SPECL [(--`P ==> R`--), (--`Q ==> R`--)] AND2_THM
+  val q_imp_r = MP my_and2 ass_rhs
+  val r_from_q = MP q_imp_r ass_Q
+  val rl_imp = DISCH rhs (DISCH porq (DISJ_CASES ass_porq r_from_p r_from_q))
+in
+  save_thm("DISJ_IMP_THM", GENL [P,Q,R] (IMP_ANTISYM_RULE lr_imp rl_imp))
+end
 
 (* ---------------------------------------------------------------------*)
 (* IMP_F_EQ_F                                                           *)
@@ -1914,9 +1946,9 @@ val _ = save_thm ("IMP_DISJ_THM", IMP_DISJ_THM);
 (* |- !t. t ==> F = (t = F)					        *)
 (*				       	                   RJB 92.09.26 *)
 (* ---------------------------------------------------------------------*)
-local fun nthCONJUNCT n cth = 
+local fun nthCONJUNCT n cth =
         let val th = funpow (n-1) CONJUNCT2 cth
-        in if (is_conj (concl th)) 
+        in if (is_conj (concl th))
            then CONJUNCT1 th else th
         end
 in
@@ -1953,7 +1985,7 @@ let val t1 = --`t1:bool`--
     and thF2 = SUBST_CONV [t1 |-> ASSUME (--`t1 = F`--)] tm tm
     val thT3 = EQ_MP (SYM thT2) thT1
     and thF3 = EQ_MP (SYM thF2) thF1
- in  
+ in
    GENL [t1,t2,t3] (DISJ_CASES (SPEC t1 BOOL_CASES_AX) thT3 thF3)
  end;
 
@@ -1987,7 +2019,7 @@ let val t1 = --`t1:bool`--
     and thF2 = SUBST_CONV [t1 |-> ASSUME (--`t1 = F`--)] tm tm
     val thT3 = EQ_MP (SYM thT2) thT1
     and thF3 = EQ_MP (SYM thF2) thF1
- in  
+ in
    GENL [t1,t2] (DISJ_CASES (SPEC t1 BOOL_CASES_AX) thT3 thF3)
  end;
 
@@ -2037,14 +2069,14 @@ val _ = save_thm("EQ_EXPAND", EQ_EXPAND);
 val COND_RATOR =
 let val f = --`f: 'a -> 'b`--
     val g = --`g: 'a -> 'b`--
-    val x = --`x:'a`--   
+    val x = --`x:'a`--
     and b = --`b:bool`--
     val fx = --`^f ^x`-- and gx = --`^g ^x`--
     val t1 = --`t1:'a`--
     val t2 = --`t2:'a`--
     val theta1 = [Type`:'a` |-> Type`:'a -> 'b`]
     val theta2 = [Type`:'a` |-> Type`:'b`]
-    val (COND_T,COND_F) = (GENL[t1,t2]##GENL[t1,t2]) 
+    val (COND_T,COND_F) = (GENL[t1,t2]##GENL[t1,t2])
                           (CONJ_PAIR(SPEC_ALL COND_CLAUSES))
     val thTl = AP_THM (SPECL [f,g] (INST_TYPE theta1 COND_T)) x
     and thFl = AP_THM (SPECL [f,g] (INST_TYPE theta1 COND_F)) x
@@ -2073,8 +2105,8 @@ val _ = save_thm("COND_RATOR", COND_RATOR);
 
 val COND_RAND =
 let val f = --`f: 'a -> 'b`--
-    val x = --`x:'a`--   
-    val y = --`y:'a`--   
+    val x = --`x:'a`--
+    val y = --`y:'a`--
     and b = --`b:bool`--
     val fx = --`^f ^x`-- and fy = --`^f ^y`--
     val t1 = --`t1:'a`--
@@ -2112,9 +2144,9 @@ let val b = --`b:bool`--
     val f = --`f:'a->'b`--
     val g = --`g:'a->'b`--
     val x = --`x:'a`--
- in 
+ in
    GENL [b,f,g]
-      (TRANS (ABS x (SYM (SPECL [b,f,g,x] COND_RATOR))) 
+      (TRANS (ABS x (SYM (SPECL [b,f,g,x] COND_RATOR)))
              (ETA_CONV (--`\^x. (^b => ^f | ^g) ^x`--)))
  end;
 
@@ -2135,7 +2167,7 @@ let val b    = --`b:bool`--
     val conj = --`$/\`--
     val disj = --`$\/`--
     val theta = [Type`:'a` |-> Type.bool]
-    val (COND_T,COND_F) = 
+    val (COND_T,COND_F) =
       let val t1 = --`t1:'a`--  and  t2 = --`t2:'a`--
       in (GENL[t1,t2]##GENL[t1,t2]) (CONJ_PAIR(SPEC_ALL COND_CLAUSES))
       end
@@ -2163,7 +2195,7 @@ let val b    = --`b:bool`--
     and thF2 = SUBST_CONV [b |-> ASSUME (--`b = F`--)] tm tm
     val thT3 = EQ_MP (SYM thT2) thT1
     and thF3 = EQ_MP (SYM thF2) thF1
- in  
+ in
    GENL [b, t1, t2] (DISJ_CASES (SPEC b BOOL_CASES_AX) thT3 thF3)
  end;
 
@@ -2174,15 +2206,15 @@ val _ = save_thm("COND_EXPAND", COND_EXPAND);
 (*---------------------------------------------------------------------------*
  * Used in basicHol90Lib.Type_def_support                                    *
  *---------------------------------------------------------------------------*)
-val ABS_REP_THM = 
-   let val th1 = ASSUME (--`?rep:'b->'a. TYPE_DEFINITION P rep`--) 
+val ABS_REP_THM =
+   let val th1 = ASSUME (--`?rep:'b->'a. TYPE_DEFINITION P rep`--)
        and th2 = MK_EXISTS (SPEC (--`P:'a->bool`--) TYPE_DEFINITION)
        val def = EQ_MP th2 th1
        val asm = ASSUME (#Body(dest_exists(concl def)))
        val (asm1,asm2)  = CONJ_PAIR asm
-       val rep_eq = 
+       val rep_eq =
          let val th1 = DISCH (--`a:'b=a'`--)
-                         (AP_TERM (--`rep:'b->'a`--) (ASSUME (--`a:'b=a'`--))) 
+                         (AP_TERM (--`rep:'b->'a`--) (ASSUME (--`a:'b=a'`--)))
          in IMP_ANTISYM_RULE (SPECL [(--`a:'b`--),(--`a':'b`--)] asm1) th1
          end
        val ABS = (--`\r:'a. @a:'b. r = rep a`--)
@@ -2198,11 +2230,11 @@ val ABS_REP_THM =
        val {lhs=t1l,rhs=t1r} = dest_eq (concl t1)
        val rep = fst(strip_comb t1r)
        val template = mk_eq{lhs=t1l, rhs = mk_comb{Rator=rep,Rand=v}}
-       val imp1 = DISCH (--`(P:'a->bool) r`--) 
+       val imp1 = DISCH (--`(P:'a->bool) r`--)
                     (SYM (SUBST [v |-> SYM absd2] template t1))
-       val t2 = EXISTS ((--`?a:'b. r:'a = rep a`--), (--`^ABS r`--)) 
+       val t2 = EXISTS ((--`?a:'b. r:'a = rep a`--), (--`^ABS r`--))
 	               (SYM(ASSUME (--`rep(^ABS (r:'a):'b) = r`--)))
-       val imp2 = DISCH (--`rep(^ABS (r:'a):'b) = r`--) 
+       val imp2 = DISCH (--`rep(^ABS (r:'a):'b) = r`--)
      		        (EQ_MP (SYM (SPEC (--`r:'a`--) asm2)) t2)
        val TH2 = GEN (--`r:'a`--) (IMP_ANTISYM_RULE imp1 imp2)
        val CTH = CONJ TH1 TH2
